Refactoring proofs and definitions

doc/coq/.CoqMakefile.d
@@ -1,24 +1,6 @@
-simple/ALinking.vo simple/ALinking.glob simple/ALinking.v.beautified simple/ALinking.required_vo: simple/ALinking.v simple/Abstract.vo
-simple/ALinking.vio: simple/ALinking.v simple/Abstract.vio
-simple/ALinking.vos simple/ALinking.vok simple/ALinking.required_vos: simple/ALinking.v simple/Abstract.vos
-simple/Abstract.vo simple/Abstract.glob simple/Abstract.v.beautified simple/Abstract.required_vo: simple/Abstract.v simple/Syntax.vo
-simple/Abstract.vio: simple/Abstract.v simple/Syntax.vio
-simple/Abstract.vos simple/Abstract.vok simple/Abstract.required_vos: simple/Abstract.v simple/Syntax.vos
 simple/Concrete.vo simple/Concrete.glob simple/Concrete.v.beautified simple/Concrete.required_vo: simple/Concrete.v simple/Syntax.vo
 simple/Concrete.vio: simple/Concrete.v simple/Syntax.vio
 simple/Concrete.vos simple/Concrete.vok simple/Concrete.required_vos: simple/Concrete.v simple/Syntax.vos
-simple/Fixpoint.vo simple/Fixpoint.glob simple/Fixpoint.v.beautified simple/Fixpoint.required_vo: simple/Fixpoint.v simple/Abstract.vo
-simple/Fixpoint.vio: simple/Fixpoint.v simple/Abstract.vio
-simple/Fixpoint.vos simple/Fixpoint.vok simple/Fixpoint.required_vos: simple/Fixpoint.v simple/Abstract.vos
-simple/LinkSound.vo simple/LinkSound.glob simple/LinkSound.v.beautified simple/LinkSound.required_vo: simple/LinkSound.v simple/ALinking.vo simple/Linking.vo
-simple/LinkSound.vio: simple/LinkSound.v simple/ALinking.vio simple/Linking.vio
-simple/LinkSound.vos simple/LinkSound.vok simple/LinkSound.required_vos: simple/LinkSound.v simple/ALinking.vos simple/Linking.vos
-simple/Linking.vo simple/Linking.glob simple/Linking.v.beautified simple/Linking.required_vo: simple/Linking.v simple/Sound.vo
-simple/Linking.vio: simple/Linking.v simple/Sound.vio
-simple/Linking.vos simple/Linking.vok simple/Linking.required_vos: simple/Linking.v simple/Sound.vos
-simple/Sound.vo simple/Sound.glob simple/Sound.v.beautified simple/Sound.required_vo: simple/Sound.v simple/Abstract.vo simple/Concrete.vo
-simple/Sound.vio: simple/Sound.v simple/Abstract.vio simple/Concrete.vio
-simple/Sound.vos simple/Sound.vok simple/Sound.required_vos: simple/Sound.v simple/Abstract.vos simple/Concrete.vos
 simple/Syntax.vo simple/Syntax.glob simple/Syntax.v.beautified simple/Syntax.required_vo: simple/Syntax.v 
 simple/Syntax.vio: simple/Syntax.v 
 simple/Syntax.vos simple/Syntax.vok simple/Syntax.required_vos: simple/Syntax.v 
