doc/coq/simple/Concrete.v
@@ -2,15 +2,10 @@ From Simple Require Export Syntax.
 
 Generalizable Variables T.
 
-Inductive state {T : Type} :=
-  | ST (mem : T -> option (@expr_value T))
-       (t : T)
-.
-
-Class time `{OrderT T} :=
-{  
-  tick : @dy_ctx T -> @state T -> expr_id -> @expr_value T -> T;
-  tick_lt : forall C mem t x v, t < tick C (ST mem t) x v
+Class time `{TotalOrder T} :=
+{
+  tick : @dy_ctx T -> @memory T -> T -> ID -> @expr_value T -> T;
+  tick_lt : forall C mem t x v, t < tick C mem t x v
 }.
 
 Definition update_m {T X} `{Eq T} mem (t : T) (x : X) :=
@@ -21,66 +16,103 @@ Definition empty_mem {T X} (t : T) : option X := None.
 Notation "p '!->' v ';' mem" := (update_m mem p v)
                               (at level 100, v at next level, right associativity).
 
-Inductive EvalR `{time T} (C : @dy_ctx T) (st : @state T)
-    : tm -> (@dy_value T) -> (@state T) -> Prop :=
-  | Eval_var_e x v mem t addr
-             (STATE : ST mem t = st)
-             (ADDR : Some addr = addr_x C x)
-             (ACCESS : Some v = mem addr)
-    : EvalR C st (e_var x) (EVal v) (ST mem t)
-  | Eval_lam x e
-    : EvalR C st (e_lam x e)
-            (EVal (Closure x e C)) st
-  | Eval_app e1 e2
-             x e C_lam st_lam
-             arg mem t
-             v st_v
-             (FN : EvalR C st e1
-                         (EVal (Closure x e C_lam)) st_lam)
-             (ARG : EvalR C st_lam e2
-                          (EVal arg) (ST mem t))
-             (BODY : EvalR (C_lam [|dy_binde x t ([||])|])
-                           (ST (t !-> arg ; mem) (tick C (ST mem t) x arg))
-                           e (EVal v) st_v)
-    : EvalR C st (e_app e1 e2) (EVal v) st_v
-  | Eval_link m e C_m st_m v st_v
-               (MOD : EvalR C st m (MVal C_m) st_m)
-               (LINK : EvalR C_m st_m e v st_v)
-    : EvalR C st (e_link m e) v st_v
-  | Eval_empty
-    : EvalR C st m_empty (MVal C) st
-  | Eval_var_m M C_M (ACCESS : Some C_M = ctx_M C M)
-    : EvalR C st (m_var M) (MVal C_M) st
-  | Eval_lete x e v mem t
-              m C_m st_m
-               (EVALe : EvalR C st e (EVal v) (ST mem t))
-               (EVALm : EvalR (C [|dy_binde x t ([||])|])
-                        (ST (t !-> v ; mem) (tick C (ST mem t) x v))
-                        m (MVal C_m) st_m)
-    : EvalR C st (m_lete x e m) (MVal C_m) st_m
-  | Eval_letm M m' C' st'
-              m'' C'' st''
-              (EVALm' : EvalR C st m' (MVal C') st')
-              (EVALm'' : EvalR (C [|dy_bindm M C' ([||])|]) st'
-                         m'' (MVal C'') st'')
-    : EvalR C st (m_letm M m' m'') (MVal C'') st''
+Inductive step `{time T} : (@config T) -> (@config T) -> Prop :=
+  | ExprID x C m t v addr
+    (ADDR : addr_x C x = Some addr)
+    (ACCESS : m addr = Some v)
+    : step (Cf (e_var x) C m t) (Rs (EVal v) m t)
+
+  | Fn x e C m t
+    : step (Cf (e_lam x e) C m t) (Rs (EVal (Closure x e C)) m t)
+
+  | AppL e1 e2 C m t
+    : step (Cf (e_app e1 e2) C m t) (Cf e1 C m t)
+
+  | AppR e1 e2 C m t x e C_f m_f t_f
+    (FN : step (Cf e1 C m t) (Rs (EVal (Closure x e C_f)) m_f t_f))
+    : step (Cf (e_app e1 e2) C m t) (Cf e2 C m_f t_f)
+
+  | AppBody e1 e2 C m t x e C_f m_f t_f v m_a t_a
+    (FN : step (Cf e1 C m t) (Rs (EVal (Closure x e C_f)) m_f t_f))
+    (ARG : step (Cf e2 C m_f t_f) (Rs (EVal v) m_a t_a))
+    : step (Cf (e_app e1 e2) C m t) (Cf e (dy_binde x t_a C_f) (t_a !-> v; m_a) (tick C m_a t_a x v))
+
+  | App e1 e2 C m t x e C_f m_f t_f v m_a t_a v' m' t'
+    (FN : step (Cf e1 C m t) (Rs (EVal (Closure x e C_f)) m_f t_f))
+    (ARG : step (Cf e2 C m_f t_f) (Rs (EVal v) m_a t_a))
+    (BODY : step (Cf e (dy_binde x t_a C_f) (t_a !-> v; m_a) (tick C m_a t_a x v)) (Rs (EVal v') m' t'))
+    : step (Cf (e_app e1 e2) C m t) (Rs (EVal v') m' t')
+
+  | LinkL e1 e2 C m t
+    : step (Cf (e_link e1 e2) C m t) (Cf e1 C m t)
+  
+  | LinkR e1 e2 C m t C' m' t'
+    (MOD : step (Cf e1 C m t) (Rs (MVal C') m' t'))
+    : step (Cf (e_link e1 e2) C m t) (Cf e2 C' m' t')
+  
+  | Link e1 e2 C m t C' m' t' V m'' t''
+    (MOD : step (Cf e1 C m t) (Rs (MVal C') m' t'))
+    (LINK : step (Cf e2 C' m' t') (Rs V m'' t''))
+    : step (Cf (e_link e1 e2) C m t) (Rs V m'' t'')
+  
+  | Empty C m t
+    : step (Cf m_empty C m t) (Rs (MVal C) m t)
+  
+  | ModID M C m t C_M
+    (ACCESS : ctx_M C M = Some C_M)
+    : step (Cf (m_var M) C m t) (Rs (MVal C_M) m t)
+  
+  | LetEL x e1 e2 C m t
+    : step (Cf (m_lete x e1 e2) C m t) (Cf e1 C m t)
+  
+  | LetER x e1 e2 C m t v m' t'
+    (EVALx : step (Cf e1 C m t) (Rs (EVal v) m' t'))
+    : step (Cf (m_lete x e1 e2) C m t) (Cf e2 (dy_binde x t' C) (t' !-> v; m') (tick C m' t' x v))
+  
+  | LetE x e1 e2 C m t v m' t' C' m'' t''
+    (EVALx : step (Cf e1 C m t) (Rs (EVal v) m' t'))
+    (EVALm : step (Cf e2 (dy_binde x t' C) (t' !-> v; m') (tick C m' t' x v)) (Rs (MVal C') m'' t''))
+    : step (Cf (m_lete x e1 e2) C m t) (Rs (MVal C') m'' t'')
+  
+  | LetML M e1 e2 C m t
+    : step (Cf (m_letm M e1 e2) C m t) (Cf e1 C m t)
+  
+  | LetMR M e1 e2 C m t C' m' t'
+    (EVALM : step (Cf e1 C m t) (Rs (MVal C') m' t'))
+    : step (Cf (m_letm M e1 e2) C m t) (Cf e2 (dy_bindm M C' C) m' t')
+
+  | LetM M e1 e2 C m t C' m' t' C'' m'' t''
+    (EVALM : step (Cf e1 C m t) (Rs (MVal C') m' t'))
+    (EVALm : step (Cf e2 (dy_bindm M C' C) m' t') (Rs (MVal C'') m'' t''))
+    : step (Cf (m_letm M e1 e2) C m t) (Rs (MVal C'') m'' t'')
 .
 
-#[export] Hint Constructors EvalR : core.
+#[export] Hint Constructors step : core.
 
-Inductive config {T} :=
-  | Config (C : @dy_ctx T) (st : @state T) (e : tm)
+Inductive multi_step `{time T} : (@config T) -> (@config T) -> Prop :=
+  | Refl cf : multi_step cf cf
+  | Trans cf cf' cf''
+    (REACHl : step cf cf')
+    (REACHr : multi_step cf' cf'')
+    : multi_step cf cf''
 .
 
-Inductive interpreter_state {T} :=
+Notation "'{|' ll '~>' rr '|}'" := 
+  (step ll rr) 
+  (at level 10, ll at next level, rr at next level).
+
+Notation "'{|' ll '~>*' rr '|}'" := 
+  (multi_step ll rr) 
+  (at level 10, ll at next level, rr at next level).
+
+Inductive interpreter_state `{time T} :=
   | Pending (reached : list (@config T))
   | Error (reached : list (@config T)) (* Type error *)
-  | Resolved (v : @dy_value T) (st : @state T) (reached : list (@config T))
+  | Resolved (V : @dy_value T) (m : @memory T) (t : T) (reached : list (@config T))
 .
 
-Fixpoint eval `{time T} (C : @dy_ctx T) (st : @state T) 
-              (e : tm) (reached : list config) (FUEL : nat) :=
-  let reached := (Config C st e) :: reached in
+Fixpoint eval `{time T} e C m t (reached : list (@config T)) (FUEL : nat) :=
+  let reached := (Cf e C m t) :: reached in
   match FUEL with
   | 0 => Pending reached
   | S FUEL' =>
@@ -89,1183 +121,513 @@ Fixpoint eval `{time T} (C : @dy_ctx T) (st : @state T)
       match addr_x C x with
       | None => Error reached
       | Some addr =>
-        match st with
-        | ST mem _ =>
-          match mem addr with
-          | None => Pending reached
-          | Some v => Resolved (EVal v) st reached
-          end
+        match m addr with
+        | None => Error reached
+        | Some v => Resolved (EVal v) m t ((Rs (EVal v) m t) :: reached)
         end
       end
-    | e_lam x e' =>
-      Resolved (EVal (Closure x e' C)) st reached
+    | e_lam x e =>
+      let v := Closure x e C in
+      Resolved (EVal v) m t ((Rs (EVal v) m t) :: reached)
     | e_app e1 e2 =>
-      match eval C st e1 reached FUEL' with
-      | Resolved (EVal (Closure x e' C_lam)) st_lam reached' =>
-        match eval C st_lam e2 reached' FUEL' with
-        | Resolved (EVal arg) (ST mem t) reached'' =>
-          match eval (C_lam [| dy_binde x t ([||]) |]) 
-                     (ST (t !-> arg ; mem) (tick C (ST mem t) x arg)) 
-                     e' reached'' FUEL' with
-          | Resolved (EVal v) st' reached''' => Resolved (EVal v) st' reached'''
-          | Resolved _ _ reached''' => Error reached'''
+      match eval e1 C m t reached FUEL' with
+      | Resolved (EVal (Closure x e C_f)) m_f t_f reached' =>
+        match eval e2 C m_f t_f reached' FUEL' with
+        | Resolved (EVal v) m_a t_a reached'' =>
+          match eval e (dy_binde x t_a C_f) (t_a !-> v; m_a) (tick C m_a t_a x v) reached'' FUEL' with
+          | Resolved (EVal v') m' t' reached''' => Resolved (EVal v') m' t' reached'''
+          | Resolved _ _ _ reached''' => Error reached'''
           | other => other
           end
-        | Resolved _ _ reached'' => Error reached''
+        | Resolved _ _ _ reached'' => Error reached''
         | other => other
         end
-      | Resolved _ _ reached' => Error reached'
+      | Resolved _ _ _ reached' => Error reached'
       | other => other
       end
-    | e_link m e' =>
-      match eval C st m reached FUEL' with
-      | Resolved (MVal C_m) st_m reached' =>
-        match eval C_m st_m e' reached' FUEL' with
-        | Resolved v st' reached'' => Resolved v st' reached''
+    | e_link e1 e2 =>
+      match eval e1 C m t reached FUEL' with
+      | Resolved (MVal C') m' t' reached' =>
+        match eval e2 C' m' t' reached' FUEL' with
+        | Resolved V m'' t'' reached'' => Resolved V m'' t'' reached''
         | other => other
         end
-      | Resolved _ _ reached' => Error reached'
+      | Resolved _ _ _ reached' => Error reached'
       | other => other
       end
-    | m_empty => Resolved (MVal C) st reached
+    | m_empty => Resolved (MVal C) m t ((Rs (MVal C) m t) :: reached)
     | m_var M =>
       match ctx_M C M with
-      | None => Pending reached
-      | Some C_M => Resolved (MVal C_M) st reached
+      | None => Error reached
+      | Some C_M => Resolved (MVal C_M) m t ((Rs (MVal C_M) m t) :: reached)
       end
-    | m_lete x e m =>
-      match eval C st e reached FUEL' with
-      | Resolved (EVal v) (ST mem t) reached' =>
-        match eval (C[| dy_binde x t ([||]) |]) 
-                   (ST (t !-> v ; mem) (tick C (ST mem t) x v)) 
-                   m reached' FUEL' with
-        | Resolved (MVal C') st' reached'' => Resolved (MVal C') st' reached''
-        | Resolved _ _ reached'' => Error reached''
+    | m_lete x e1 e2 =>
+      match eval e1 C m t reached FUEL' with
+      | Resolved (EVal v) m' t' reached' =>
+        match eval e2 (dy_binde x t' C) (t' !-> v; m') (tick C m' t' x v) reached' FUEL' with
+        | Resolved (MVal C') m'' t'' reached'' => Resolved (MVal C') m'' t'' reached''
+        | Resolved _ _ _ reached'' => Error reached''
         | other => other
         end
-      | Resolved _ _ reached' => Error reached'
+      | Resolved _ _ _ reached' => Error reached'
       | other => other
       end
-    | m_letm M m1 m2 =>
-      match eval C st m1 reached FUEL' with
-      | Resolved (MVal C') st' reached' =>
-        match eval (C[| dy_bindm M C' ([||]) |])
-                   st' m2 reached' FUEL' with
-        | Resolved (MVal C'') st'' reached'' => Resolved (MVal C'') st'' reached''
-        | Resolved _ _ reached'' => Error reached''
+    | m_letm M e1 e2 =>
+      match eval e1 C m t reached FUEL' with
+      | Resolved (MVal C') m' t' reached' =>
+        match eval e2 (dy_bindm M C' C) m' t' reached' FUEL' with
+        | Resolved (MVal C'') m'' t'' reached'' => Resolved (MVal C'') m'' t'' reached''
+        | Resolved _ _ _ reached'' => Error reached''
         | other => other
         end
-      | Resolved _ _ reached' => Error reached'
+      | Resolved _ _ _ reached' => Error reached'
       | other => other
       end
     end
   end.
 
-Lemma relax_fuel :
-  forall `{TIME : time T} (C : @dy_ctx T) st e l l' v st' FUEL FUEL' (LE : FUEL <= FUEL'),
-    eval C st e l FUEL = Resolved v st' l' ->
-    eval C st e l FUEL' = Resolved v st' l'.
+Ltac rep_eval SOLVER :=
+  match goal with
+  | [RR : eval ?e ?C ?m ?t ?l ?n = _ |- 
+          context [eval ?e ?C ?m ?t ?l ?n]] =>
+    (* trivial case *)
+    rewrite RR;
+    move RR at top
+  | [RR : eval ?e ?C ?m ?t ?l ?n = _ |-
+      context [eval ?e ?C ?m ?t ?l ?n0]] =>
+    (* relaxation *)
+    replace (eval e C m t l n0) with (eval e C m t l n);
+    rewrite RR;
+    (* IHFUEL *)
+    try (symmetry; apply SOLVER; eauto; fail);
+    (* relax_fuel *)
+    try (symmetry; apply SOLVER with (FUEL := n); try nia; eauto; fail);
+    move RR at top
+  | [RR : eval ?e ?C ?m ?t ?l ?n = _ |-
+      context [eval ?e ?C ?m ?t ?l0 ?n0]] =>
+    (* relaxation, l is an evar *)
+    replace (eval e C m t l0 n0) with (eval e C m t l n);
+    rewrite RR;
+    (* IHFUEL *)
+    try (symmetry; apply SOLVER; eauto; fail);
+    (* relax_fuel *)
+    try (symmetry; apply SOLVER with (FUEL := n); try nia; eauto; fail);
+    move RR at top
+  | _ => fail
+  end.
+
+Lemma relax_fuel `{time T} :
+  forall FUEL FUEL' (LE : FUEL <= FUEL') e C m t l l' V m' t'
+    (EVAL : eval e C m t l FUEL = Resolved V m' t' l'),
+    eval e C m t l FUEL' = Resolved V m' t' l'.
 Proof.
-  intros. rename H into H'. rename H0 into H''. rename H1 into H.
-  revert C st e l l' v st' H FUEL' LE.
+  rename H into ET. rename H0 into OT. rename H1 into TT.
   induction FUEL; intros.
-  - inversion H.
-  - simpl in H; destruct e; inversion LE; eauto.
-    + remember (eval C st e1 (Config C st (e_app e1 e2) :: l) FUEL) as v1.
-      destruct v1 as [ | | v1 st1]; inversion H.
-      clear H3. destruct v1 as [v1 | ]; inversion H.
-      clear H3. destruct v1 as [x v1 C_lam].
-      remember (eval C st1 e2 reached FUEL) as v2.
-      destruct v2 as [ | | v2 st2]; inversion H;
-      clear H3. destruct v2 as [v2 | ]; inversion H.
-      clear H3. destruct st2 as [mem2 t2].
-      remember (eval (C_lam [|dy_binde x t2 ([||])|]) 
-                     (ST (t2 !-> v2; mem2) (tick C (ST mem2 t2) x v2))
-                      v1 reached0 FUEL) as v3.
-      destruct v3 as [ | | v3 st3]; inversion H.
-      clear H3. destruct v3 as [v3 | ]; inversion H.
-      subst. 
-      assert (eval C st e1 (Config C st (e_app e1 e2) :: l) m = Resolved (EVal (Closure x v1 C_lam)) st1 reached) as RR1.
-      apply IHFUEL; eauto. nia.
-      assert (eval C st1 e2 reached m = Resolved (EVal v2) (ST mem2 t2) reached0) as RR2.
-      apply IHFUEL; eauto. nia.
-      assert (eval (C_lam [|dy_binde x t2 ([||])|])
-                   (ST (t2 !-> v2; mem2) (tick C (ST mem2 t2) x v2)) v1 reached0 m = 
-              Resolved (EVal v3) st' l') as RR3.
-      apply IHFUEL; eauto. nia.
-      simpl. rewrite RR1. rewrite RR2. rewrite RR3. eauto.
-    + remember (eval C st e1 (Config C st (e_link e1 e2) :: l) FUEL) as v1.
-      destruct v1 as [ | | v1 st1]; inversion H.
-      clear H3. destruct v1 as [v1 | ]; inversion H.
-      remember (eval mv st1 e2 reached FUEL) as v2.
-      clear H3. destruct v2 as [ | | v2 st2]; inversion H.
-      clear H3. destruct v2 as [v2 | ]; inversion H; subst;
-      assert (eval C st e1 (Config C st (e_link e1 e2) :: l) m = Resolved (MVal mv) st1 reached) as RR1;
-      try (apply IHFUEL; eauto; nia).
-      assert (eval mv st1 e2 reached m = Resolved (EVal v2) st' l') as RR2.
-      apply IHFUEL; eauto; nia.
-      simpl. rewrite RR1. rewrite RR2. eauto.
-      assert (eval mv st1 e2 reached m = Resolved (MVal mv0) st' l') as RR2.
-      apply IHFUEL; eauto; nia.
-      simpl. rewrite RR1. rewrite RR2. eauto.
-    + remember (eval C st e1 (Config C st (m_lete x e1 e2) :: l) FUEL) as v1.
-      destruct v1 as [ | | v1 st1]; inversion H.
-      clear H3. destruct v1 as [v1 | ]; inversion H.
-      clear H3. destruct st1 as [mem1 t1].
-      remember (eval (C [|dy_binde x t1 ([||])|]) 
-                     (ST (t1 !-> v1; mem1) (tick C (ST mem1 t1) x v1))
-                      e2 reached FUEL) as v2.
-      destruct v2 as [ | | v2 st2]; inversion H.
-      clear H3. destruct v2 as [v2 | ]; inversion H.
-      subst.
-      assert (eval C st e1 (Config C st (m_lete x e1 e2) :: l) m = Resolved (EVal v1) (ST mem1 t1) reached) as RR1.
-      apply IHFUEL; eauto. nia.
-      assert (eval (C [|dy_binde x t1 ([||])|]) 
-                   (ST (t1 !-> v1; mem1) (tick C (ST mem1 t1) x v1))
-                   e2 reached m = Resolved (MVal mv) st' l') as RR2.
-      apply IHFUEL; eauto. nia.
-      simpl. rewrite RR1. rewrite RR2. eauto.
-    + remember (eval C st e1 (Config C st (m_letm M e1 e2) :: l) FUEL) as v1.
-      destruct v1 as [ | | v1 st1]; inversion H.
-      clear H3. destruct v1 as [v1 | ]; inversion H.
-      clear H3.
-      remember (eval (C [|dy_bindm M mv ([||])|]) st1
-                      e2 reached FUEL) as v2.
-      destruct v2 as [ | | v2 st2]; inversion H.
-      clear H3. destruct v2 as [v2 | ]; inversion H.
-      subst.
-      assert (eval C st e1 (Config C st (m_letm M e1 e2) :: l) m = Resolved (MVal mv) st1 reached) as RR1.
-      apply IHFUEL; eauto. nia.
-      assert (eval (C [|dy_bindm M mv ([||])|]) st1
-                   e2 reached m = Resolved (MVal mv0) st' l') as RR2.
-      apply IHFUEL; eauto. nia.
-      simpl. rewrite RR1. rewrite RR2. eauto.
+  - inversion EVAL.
+  - inversion LE; eauto. 
+    assert (FUEL <= m0) as HINT. { nia. }
+    specialize (IHFUEL m0 HINT).
+    destruct e; simpl in *; eauto; repeat des_hyp;
+    rep_eval IHFUEL;
+    rep_eval IHFUEL; eauto.
+    rep_eval IHFUEL. eauto.
 Qed.
-      
-Lemma EvalR_well_defined_l :
-  forall `{time T} (C : @dy_ctx T) st e l v st' (R : EvalR C st e v st'),
+
+Lemma relax_fuel_err `{time T} :
+  forall FUEL FUEL' (LE : FUEL <= FUEL') e C m t l l'
+    (EVAL : eval e C m t l FUEL = Error l'),
+    eval e C m t l FUEL' = Error l'.
+Proof.
+  rename H into ET. rename H0 into OT. rename H1 into TT.
+  induction FUEL; intros.
+  inversion EVAL.
+  inversion LE; eauto. 
+  assert (FUEL <= m0) as HINT. { nia. }
+  specialize (IHFUEL m0 HINT).
+  destruct e; simpl in *; eauto; repeat des_hyp;
+  try (erewrite IHFUEL; eauto; fail);
+  try (erewrite relax_fuel; eauto);
+  simpl; eauto;
+  try (rep_eval IHFUEL; eauto; fail);
+  try (rep_eval relax_fuel; eauto; fail).
+  rep_eval relax_fuel. rep_eval IHFUEL. eauto.
+  rep_eval relax_fuel. rep_eval relax_fuel. eauto.
+Qed.
+
+Lemma Eval_well_defined_l :
+  forall `{time T} e (C : @dy_ctx T) m t l V m' t' 
+    (R : {| Cf e C m t ~> Rs V m' t' |}),
     exists FUEL, 
-      match eval C st e l FUEL with
-      | Resolved v' st'' _ => v = v' /\ st' = st''
+      match eval e C m t l FUEL with
+      | Resolved V' m'' t'' _ => V = V' /\ m' = m'' /\ t' = t''
       | _ => False
       end.
 Proof.
-  intros. revert l. induction R; intros.
-  - exists 1; simpl. rewrite <- ADDR. rewrite <- STATE. rewrite <- ACCESS. eauto.
+  intros. revert l. remember (Cf e C m t) as cf. remember (Rs V m' t') as rs.
+  generalize dependent e. generalize dependent V. revert C m t m' t'.
+  induction R; intros; inversion Heqcf; inversion Heqrs; subst.
+  - exists 1; simpl. rewrite ADDR. rewrite ACCESS. eauto.
   - exists 1; simpl; eauto.
-  - destruct (IHR1 (Config C st (e_app e1 e2) :: l)) as [FUEL' EQ']. clear IHR1.
-    destruct (eval C st e1 (Config C st (e_app e1 e2) :: l) FUEL') eqn:EVAL1; try (inversion EQ'; fail).
-    destruct (IHR2 reached) as [FUEL'' EQ'']. clear IHR2.
-    destruct (eval C st_lam e2 reached FUEL'') eqn:EVAL2; try (inversion EQ''; fail).
-    destruct (IHR3 reached0) as [FUEL''' EQ''']. clear IHR3.
-    destruct (eval (C_lam [|dy_binde x t ([||])|])
-                   (ST (t !-> arg; mem) (tick C (ST mem t) x arg)) e reached0
-                   FUEL''') eqn:EVAL3; try (inversion EQ'''; fail).
+  - edestruct IHR1 as [FUEL' EQ']; eauto. clear IHR1. des_hyp.
+    edestruct IHR2 as [FUEL'' EQ'']; eauto. clear IHR2. des_hyp.
+    edestruct IHR3 as [FUEL''' EQ''']; eauto. clear IHR3. des_hyp.
     exists (S (Nat.max FUEL' (Nat.max FUEL'' FUEL'''))).
     simpl.
-    destruct EQ' as [RR RR']. rewrite <- RR in *. rewrite <- RR' in *. clear RR RR'.
-    destruct EQ'' as [RR RR']. rewrite <- RR in *. rewrite <- RR' in *. clear RR RR'.
-    destruct EQ''' as [RR RR']. rewrite <- RR in *. rewrite <- RR' in *. clear RR RR'.
-    assert (eval C st e1 (Config C st (e_app e1 e2) :: l) (Nat.max FUEL' (Nat.max FUEL'' FUEL'''))
-            = Resolved (EVal (Closure x e C_lam)) st_lam reached) as RR.
-    apply relax_fuel with (FUEL := FUEL'). nia. eauto.
-    rewrite RR; clear RR.
-    assert (eval C st_lam e2 reached (Nat.max FUEL' (Nat.max FUEL'' FUEL'''))
-            = Resolved (EVal arg) (ST mem t) reached0) as RR.
-    apply relax_fuel with (FUEL := FUEL''). nia. eauto.
-    rewrite RR; clear RR.
-    assert (eval (C_lam [|dy_binde x t ([||])|]) 
-                 (ST (t !-> arg; mem) (tick C (ST mem t) x arg)) e reached0
-                 (Nat.max FUEL' (Nat.max FUEL'' FUEL'''))
-            = Resolved (EVal v) st_v reached1) as RR.
-    apply relax_fuel with (FUEL := FUEL'''). nia. eauto.
-    rewrite RR; clear RR. eauto.
-  - destruct (IHR1 (Config C st (e_link m e) :: l)) as [FUEL' EQ']. clear IHR1.
-    destruct (eval C st m (Config C st (e_link m e) :: l) FUEL') eqn:EVAL1; try (inversion EQ'; fail).
-    destruct (IHR2 reached) as [FUEL'' EQ'']. clear IHR2.
-    destruct (eval C_m st_m e reached FUEL'') eqn:EVAL2; try (inversion EQ''; fail).
+    destruct EQ' as [? [? ?]]. subst.
+    destruct EQ'' as [? [? ?]]. subst.
+    destruct EQ''' as [? [? ?]]. subst.
+    rep_eval relax_fuel.
+    rep_eval relax_fuel.
+    rep_eval relax_fuel. eauto.
+  - edestruct IHR1 as [FUEL' EQ']; eauto. clear IHR1. des_hyp.
+    edestruct IHR2 as [FUEL'' EQ'']; eauto. clear IHR2. des_hyp.
     exists (S (Nat.max FUEL' FUEL'')).
     simpl.
-    destruct EQ' as [RR RR']. rewrite <- RR in *. rewrite <- RR' in *. clear RR RR'.
-    destruct EQ'' as [RR RR']. rewrite <- RR in *. rewrite <- RR' in *. clear RR RR'.
-    assert (eval C st m (Config C st (e_link m e) :: l) (Nat.max FUEL' FUEL'')
-            = Resolved (MVal C_m) st_m reached) as RR.
-    apply relax_fuel with (FUEL := FUEL'). nia. eauto.
-    rewrite RR; clear RR.
-    assert (eval C_m st_m e reached (Nat.max FUEL' FUEL'')
-            = Resolved v st_v reached0) as RR.
-    apply relax_fuel with (FUEL := FUEL''). nia. eauto.
-    rewrite RR; clear RR. eauto.
-  - exists 1. simpl; eauto. 
-  - exists 1; simpl. rewrite <- ACCESS. eauto.
-  - destruct (IHR1 (Config C st (m_lete x e m) :: l)) as [FUEL' EQ']. clear IHR1.
-    destruct (eval C st e (Config C st (m_lete x e m) :: l) FUEL') eqn:EVAL1; try (inversion EQ'; fail).
-    destruct (IHR2 reached) as [FUEL'' EQ'']. clear IHR2.
-    destruct (eval (C [|dy_binde x t ([||])|])
-                   (ST (t !-> v; mem) (tick C (ST mem t) x v)) m reached
-                   FUEL'') eqn:EVAL2; try (inversion EQ''; fail).
+    destruct EQ' as [? [? ?]]. subst.
+    destruct EQ'' as [? [? ?]]. subst.
+    rep_eval relax_fuel.
+    rep_eval relax_fuel. eauto.
+  - exists 1. simpl; eauto.
+  - exists 1; simpl. rewrite ACCESS. eauto.
+  - edestruct IHR1 as [FUEL' EQ']; eauto. clear IHR1. des_hyp.
+    edestruct IHR2 as [FUEL'' EQ'']; eauto. clear IHR2. des_hyp.
     exists (S (Nat.max FUEL' FUEL'')).
     simpl.
-    destruct EQ' as [RR RR']. rewrite <- RR in *. rewrite <- RR' in *. clear RR RR'.
-    destruct EQ'' as [RR RR']. rewrite <- RR in *. rewrite <- RR' in *. clear RR RR'.
-    assert (eval C st e (Config C st (m_lete x e m) :: l) (Nat.max FUEL' FUEL'')
-            = Resolved (EVal v) (ST mem t) reached) as RR.
-    apply relax_fuel with (FUEL := FUEL'). nia. eauto.
-    rewrite RR; clear RR.
-    assert (eval (C [|dy_binde x t ([||])|]) 
-                 (ST (t !-> v; mem) (tick C (ST mem t) x v)) m reached
-                 (Nat.max FUEL' FUEL'')
-            = Resolved (MVal C_m) st_m reached0) as RR.
-    apply relax_fuel with (FUEL := FUEL''). nia. eauto.
-    rewrite RR; clear RR. eauto.
-  - destruct (IHR1 (Config C st (m_letm M m' m'') :: l)) as [FUEL' EQ']. clear IHR1.
-    destruct (eval C st m' (Config C st (m_letm M m' m'') :: l) FUEL') eqn:EVAL1; try (inversion EQ'; fail).
-    destruct (IHR2 reached) as [FUEL'' EQ'']. clear IHR2.
-    destruct (eval (C [|dy_bindm M C' ([||])|]) st' m'' reached FUEL'') eqn:EVAL2; try (inversion EQ''; fail).
+    destruct EQ' as [? [? ?]]. subst.
+    destruct EQ'' as [? [? ?]]. subst.
+    rep_eval relax_fuel.
+    rep_eval relax_fuel. eauto.
+  - edestruct IHR1 as [FUEL' EQ']; eauto. clear IHR1. des_hyp.
+    edestruct IHR2 as [FUEL'' EQ'']; eauto. clear IHR2. des_hyp.
     exists (S (Nat.max FUEL' FUEL'')).
     simpl.
-    destruct EQ' as [RR RR']. rewrite <- RR in *. rewrite <- RR' in *. clear RR RR'.
-    destruct EQ'' as [RR RR']. rewrite <- RR in *. rewrite <- RR' in *. clear RR RR'.
-    assert (eval C st m' (Config C st (m_letm M m' m'') :: l) (Nat.max FUEL' FUEL'')
-            = Resolved (MVal C') st' reached) as RR.
-    apply relax_fuel with (FUEL := FUEL'). nia. eauto.
-    rewrite RR; clear RR.
-    assert (eval (C [|dy_bindm M C' ([||])|]) st' m'' reached (Nat.max FUEL' FUEL'')
-            = Resolved (MVal C'') st'' reached0) as RR.
-    apply relax_fuel with (FUEL := FUEL''). nia. eauto.
-    rewrite RR; clear RR. eauto.
+    destruct EQ' as [? [? ?]]. subst.
+    destruct EQ'' as [? [? ?]]. subst.
+    rep_eval relax_fuel.
+    rep_eval relax_fuel. eauto.
 Qed.
 
-Lemma EvalR_well_defined_r :
-  forall `{TIME : time T} FUEL (C : @dy_ctx T) st e l v st'
-    (R : match eval C st e l FUEL with
-         | Resolved v' st'' _ => v = v' /\ st' = st''
+Ltac interp_to_rel SOLVER :=
+  match goal with
+  | [H : eval ?e ?C ?m ?t ?reached _ = Resolved ?V ?m0 ?t0 _ |- _] =>
+    let REL := fresh "REL" in
+    assert (REL : {| Cf e C m t ~> Rs V m0 t0 |});
+    try (apply SOLVER with (l := reached); rewrite H; eauto);
+    move H at top
+  | _ => fail
+  end.
+
+Lemma Eval_well_defined_r `{time T} :
+  forall FUEL (C : @dy_ctx T) m t e l V m' t'
+    (R : match eval e C m t l FUEL with
+         | Resolved V' m'' t'' _ => V = V' /\ m' = m'' /\ t' = t''
          | _ => False
          end),
-    EvalR C st e v st'.
+    {| (Cf e C m t) ~> (Rs V m' t') |}.
 Proof.
-  intros. rename H into H'. rename H0 into H''. generalize dependent T. revert e.
+  rename H into ET. rename H0 into OT. rename H1 into TT.
   induction FUEL; intros; simpl in *; try (inversion R; fail).
-  destruct e.
-  - destruct (addr_x C x) eqn:ADDR;
-    destruct st; destruct (mem t) eqn:ACCESS; 
-    inversion R. subst. eauto.
-  - inversion R. subst. eauto.
-  - remember (eval C st e1 (Config C st (e_app e1 e2) :: l) FUEL) as v1.
-    destruct v1 as [ | | v1 st1]; try inversion R.
-    destruct v1 as [v1 | ]; try inversion R.
-    destruct v1 as [x v1 C_lam].
-    remember (eval C st1 e2 reached FUEL) as v2.
-    destruct v2 as [ | | v2 st2]; try inversion R.
-    destruct v2 as [v2 | ]; try inversion R.
-    destruct st2 as [mem2 t2].
-    remember (eval (C_lam [|dy_binde x t2 ([||])|])
-                   (ST (t2 !-> v2; mem2) (tick C (ST mem2 t2) x v2)) 
-                   v1 reached0 FUEL) as v3.
-    destruct v3 as [ | | v3 st3]; try inversion R.
-    destruct v3 as [v3 | ]; try inversion R.
-    subst.
-    assert (EvalR C st e1 (EVal (Closure x v1 C_lam)) st1) as RR1. 
-    eapply IHFUEL; rewrite <- Heqv1; eauto.
-    assert (EvalR C st1 e2 (EVal v2) (ST mem2 t2)) as RR2.
-    eapply IHFUEL; rewrite <- Heqv2; eauto.
-    assert (EvalR (C_lam [|dy_binde x t2 ([||])|])
-                  (ST (t2 !-> v2; mem2) (tick C (ST mem2 t2) x v2)) v1
-            (EVal v3) st3) as RR3. 
-    eapply IHFUEL; rewrite <- Heqv3; eauto. eauto.
-  - remember (eval C st e1 (Config C st (e_link e1 e2) :: l) FUEL) as v1.
-    destruct v1 as [ | | v1 st1]; try inversion R.
-    destruct v1 as [v1 | ]; try inversion R.
-    remember (eval mv st1 e2 reached FUEL) as v2.
-    destruct v2 as [ | | v2 st2]; inversion R.
-    assert (EvalR C st e1 (MVal mv) st1).
-    eapply IHFUEL; rewrite <- Heqv1; eauto.
-    assert (EvalR mv st1 e2 v2 st2).
-    eapply IHFUEL; rewrite <- Heqv2; eauto.
-    subst. eauto.
-  - inversion R; subst. eapply Eval_empty; eauto.
-  - remember (ctx_M C M) as ACCESS.
-    destruct ACCESS; inversion R; subst. eapply Eval_var_m; eauto.
-  - remember (eval C st e1 (Config C st (m_lete x e1 e2) :: l) FUEL) as v1.
-    destruct v1 as [ | | v1 st1]; try inversion R.
-    destruct v1 as [v1 | ]; try inversion R.
-    destruct st1 as [mem1 t1].
-    remember (eval (C [|dy_binde x t1 ([||])|])
-                   (ST (t1 !-> v1; mem1) (tick C (ST mem1 t1) x v1)) 
-                   e2 reached FUEL) as v2.
-    destruct v2 as [ | | v2 st2]; try inversion R.
-    destruct v2 as [v2 | ]; inversion R.
-    assert (EvalR C st e1 (EVal v1) (ST mem1 t1)).
-    eapply IHFUEL; rewrite <- Heqv1; eauto.
-    assert (EvalR (C [|dy_binde x t1 ([||])|])
-                  (ST (t1 !-> v1; mem1) (tick C (ST mem1 t1) x v1)) e2
-            (MVal mv) st2).
-    eapply IHFUEL; rewrite <- Heqv2; eauto.
-    subst. eauto.
-  - remember (eval C st e1 (Config C st (m_letm M e1 e2) :: l) FUEL) as v1.
-    destruct v1 as [ | | v1 st1]; try inversion R.
-    destruct v1 as [v1 | ]; try inversion R.
-    remember (eval (C [|dy_bindm M mv ([||])|]) st1 e2 reached FUEL) as v2.
-    destruct v2 as [ | | v2 st2]; try inversion R.
-    destruct v2 as [v2 | ]; inversion R.
-    assert (EvalR C st e1 (MVal mv) st1).
-    eapply IHFUEL; rewrite <- Heqv1; eauto.
-    assert (EvalR (C [|dy_bindm M mv ([||])|]) st1 e2 (MVal mv0) st2).
-    eapply IHFUEL; rewrite <- Heqv2; eauto.
-    subst. eauto.
+  destruct e; repeat des_hyp;
+  destruct R as [? [? ?]]; subst; eauto;
+  inversion HDES; subst; eauto;
+  interp_to_rel IHFUEL; eauto;
+  interp_to_rel IHFUEL; eauto;
+  interp_to_rel IHFUEL; eauto.
 Qed.
 
-Theorem EvalR_well_defined :
-  forall `{TIME : time T} l C st e v st',
+Theorem Eval_well_defined `{time T} :
+  forall l e C m t V m' t',
     (exists FUEL, 
-      match eval C st e l FUEL with 
-      | Resolved v' st'' _ => v = v' /\ st' = st''
+      match eval e C m t l FUEL with 
+      | Resolved V' m'' t'' _ => V = V' /\ m' = m'' /\ t' = t''
       | _ => False
       end) <->
-    EvalR C st e v st'.
+    ({| (Cf e C m t) ~> (Rs V m' t') |}).
 Proof.
-  intros; split; try apply EvalR_well_defined_l.
-  intros. destruct H1 as [FUEL EVAL].
-  eapply EvalR_well_defined_r. eauto.
+  intros; split; try apply Eval_well_defined_l.
+  intros RR. destruct RR as [FUEL EVAL].
+  eapply Eval_well_defined_r. eauto.
 Qed.
 
-(* Reachability relation *)
-Inductive one_reach `{time T} (C : dy_ctx) (st : state)
-    : tm -> (@dy_ctx T) -> (@state T) -> tm -> Prop :=
-  | one_appl e1 e2
-    : one_reach C st (e_app e1 e2) 
-                C st e1
-  | one_appr e1 e2 x e C_lam st_lam
-             (FN : EvalR C st e1 
-                  (EVal (Closure x e C_lam)) st_lam)
-    : one_reach C st (e_app e1 e2)
-                C st_lam e2
-  | one_appbody e1 e2 x e C_lam st_lam
-                arg mem t
-                (FN : EvalR C st e1 
-                            (EVal (Closure x e C_lam)) st_lam)
-                (ARG : EvalR C st_lam e2
-                             (EVal arg) (ST mem t))
-    : one_reach C st (e_app e1 e2)
-                (C_lam[|dy_binde x t ([||])|]) 
-                (ST (t !-> arg ; mem) (tick C (ST mem t) x arg)) e
-  | one_linkl m e
-    : one_reach C st (e_link m e)
-                C st m
-  | one_linkr m e C_m st_m
-              (MOD : EvalR C st m (MVal C_m) st_m)
-    : one_reach C st (e_link m e)
-                C_m st_m e
-  | one_letel x e m
-    : one_reach C st (m_lete x e m)
-                C st e
-  | one_leter x e m v mem t
-              (EVALx : EvalR C st e (EVal v) (ST mem t))
-    : one_reach C st (m_lete x e m)
-                (C[|dy_binde x t ([||])|])
-                (ST (t !-> v ; mem) (tick C (ST mem t) x v)) m
-  | one_letml M m1 m2
-    : one_reach C st (m_letm M m1 m2)
-                C st m1
-  | one_letmr M m1 m2 C_M st_M
-              (EVALM : EvalR C st m1 (MVal C_M) st_M)
-    : one_reach C st (m_letm M m1 m2)
-                (C[|dy_bindm M C_M ([||])|]) st_M m2
-.
-
-Inductive multi_reach `{time T} (C : dy_ctx) (st : state)
-    : tm -> (@dy_ctx T) -> (@state T) -> tm -> Prop :=
-  | multi_refl e : multi_reach C st e C st e
-  | multi_step e C' st' e' C'' st'' e''
-               (REACHl : one_reach C st e C' st' e')
-               (REACHr : multi_reach C' st' e' C'' st'' e'')
-    : multi_reach C st e C'' st'' e''
-.
-
-Inductive ReachR `{time T} (C : @dy_ctx T) (st : @state T)
-    : tm -> (@dy_ctx T) -> (@state T) -> tm -> Prop :=
-  | r_refl e
-    : ReachR C st e 
-             C st e
-  | r_app_left e1 e2 C' st' e'
-               (REACHl : ReachR C st e1
-                                C' st' e')
-    : ReachR C st (e_app e1 e2) 
-             C' st' e'
-  | r_app_right e1 e2 x e C_lam st_lam C' st' e'
-                (FN : EvalR C st e1 
-                            (EVal (Closure x e C_lam)) st_lam)
-                (REACHr : ReachR C st_lam e2
-                                 C' st' e')
-    : ReachR C st (e_app e1 e2)
-             C' st' e'
-  | r_app_body e1 e2 x e C_lam st_lam
-                arg mem t
-                C' st' e'
-                (FN : EvalR C st e1 
-                            (EVal (Closure x e C_lam)) st_lam)
-                (ARG : EvalR C st_lam e2
-                             (EVal arg) (ST mem t))
-                (REACHb : ReachR (C_lam[|dy_binde x t ([||])|]) 
-                                 (ST (t !-> arg ; mem) (tick C (ST mem t) x arg)) e
-                                 C' st' e')
-    : ReachR C st (e_app e1 e2)
-             C' st' e'
-  | r_link_m m e C' st' e'
-              (REACHm : ReachR C st m
-                               C' st' e')
-    : ReachR C st (e_link m e)
-             C' st' e'
-  | r_link_e m e C_m st_m C' st' e'
-             (MOD : EvalR C st m (MVal C_m) st_m)
-             (REACHe : ReachR C_m st_m e
-                              C' st' e')
-    : ReachR C st (e_link m e)
-             C' st' e'
-  | r_lete_e x e m C' st' e'
-             (REACHe : ReachR C st e
-                              C' st' e')
-    : ReachR C st (m_lete x e m)
-             C' st' e'
-  | r_lete_m x e m v mem t
-             C' st' e'
-             (EVALx : EvalR C st e (EVal v) (ST mem t))
-             (REACHm : ReachR (C[|dy_binde x t ([||])|])
-                              (ST (t !-> v ; mem) (tick C (ST mem t) x v)) m
-                              C' st' e')
-    : ReachR C st (m_lete x e m)
-             C' st' e'
-  | r_letm_m1 M m1 m2 C' st' e'
-              (REACHm : ReachR C st m1
-                               C' st' e')
-    : ReachR C st (m_letm M m1 m2)
-             C' st' e'
-  | r_letm_m2 M m1 m2 C_M st_M
-              C' st' e'
-              (EVALM : EvalR C st m1 (MVal C_M) st_M)
-              (REACHm : ReachR (C[|dy_bindm M C_M ([||])|]) st_M m2
-                               C' st' e')
-    : ReachR C st (m_letm M m1 m2)
-             C' st' e'
-.
-
-#[export] Hint Constructors ReachR : core.
-
-Notation "'<|' C1 st1 tm1 '~>' C2 st2 tm2 '|>'" := (ReachR C1 st1 tm1 C2 st2 tm2) 
-                                               (at level 10, 
-                                                C1 at next level, st1 at next level, tm1 at next level,
-                                                C2 at next level, st2 at next level, tm2 at next level).
-
-Notation "'<|' C1 st1 tm1 '~>*' C2 st2 tm2 '|>'" := (multi_reach C1 st1 tm1 C2 st2 tm2) 
-                                               (at level 10, 
-                                                C1 at next level, st1 at next level, tm1 at next level,
-                                                C2 at next level, st2 at next level, tm2 at next level).
-
-(* sanity check *)
-Lemma reach_trans : forall {T} `{time T} (C1 : @dy_ctx T) st1 e1
-                         C2 st2 e2
-                         C3 st3 e3
-                         (REACH1 : <| C1 st1 e1 ~> C2 st2 e2 |>)
-                         (REACH2 : <| C2 st2 e2 ~> C3 st3 e3 |>),
-                         <| C1 st1 e1 ~> C3 st3 e3 |>.
-Proof.
-  intros. generalize dependent e3.
-  revert C3 st3.
-  induction REACH1; eauto.
-Qed.
-
-
-Lemma reach_eq `{time T} :
-  forall (C1 : @dy_ctx T) st1 e1 C2 st2 e2,
-  <| C1 st1 e1 ~> C2 st2 e2 |> <-> <| C1 st1 e1 ~>* C2 st2 e2 |>.
-Proof.
-  intros; split; intro REACH; induction REACH; eauto;
-  try apply multi_refl;
-  try (eapply multi_step; eauto).
-  - apply one_appl.
-  - eapply one_appr; eauto.
-  - eapply one_appbody; eauto.
-  - eapply one_linkl; eauto.
-  - eapply one_linkr; eauto.
-  - eapply one_letel; eauto.
-  - eapply one_leter; eauto.
-  - eapply one_letml; eauto.
-  - eapply one_letmr; eauto.
-  - destruct REACHl; eauto.
-Qed.
-
-Definition extract_reached {T} (interp : @interpreter_state T) :=
+Definition extract_reached `{time T} (interp : interpreter_state) :=
   match interp with
   | Pending reached
   | Error reached
-  | Resolved _ _ reached => reached
+  | Resolved _ _ _ reached => reached
   end.
 
-Lemma reach_myself :
-  forall `{TIME : time T} (C : @dy_ctx T) st e l FUEL,
-    In (Config C st e) (extract_reached (eval C st e l FUEL)) /\
-    (forall cf, In cf l -> In cf (extract_reached (eval C st e l FUEL))).
+(* replace a shorter expression with a longer expression,
+   which is rewritten with RR to be finished off with KILLER *)
+Ltac rep_with_rew short KILLER :=
+  match goal with
+  | [RR : _ = Pending short |- _] =>
+    replace short with (extract_reached (Pending short));
+    try reflexivity; rewrite <- RR
+  | [RR : Pending short = _ |- _] =>
+    replace short with (extract_reached (Pending short));
+    try reflexivity; rewrite RR
+  | [RR : _ = Error short |- _] =>
+    replace short with (extract_reached (Error short));
+    try reflexivity; rewrite <- RR
+  | [RR : Error short = _ |- _] =>
+    replace short with (extract_reached (Error short));
+    try reflexivity; rewrite RR
+  | [RR : _ = Resolved ?V ?m ?t short |- _] =>
+    replace short with (extract_reached (Resolved V m t short));
+    try reflexivity; rewrite <- RR
+  | [RR : Resolved ?V ?m ?t short = _ |- _] =>
+    replace short with (extract_reached (Resolved V m t short));
+    try reflexivity; rewrite RR
+  | [RR : _ = short |- _] =>
+    rewrite <- RR
+  | [RR : short = _ |- _] =>
+    rewrite RR
+  | _ => fail
+  end;
+  match goal with
+  | _ => apply KILLER; try right; simpl; eauto
+  | _ => fail
+  end.
+
+Lemma reach_myself `{time T} :
+  forall FUEL e (C : @dy_ctx T) m t l cf,
+    In cf (Cf e C m t :: l) -> In cf (extract_reached (eval e C m t l FUEL)).
 Proof.
-  intros. rename H into H'. rename H0 into H''.
-  revert C st e l; induction FUEL; intros; try (simpl; eauto; fail).
-  split.
-  - simpl. destruct e.
-    + destruct (addr_x C x) as [addr | ]; try destruct st;
-      try destruct (mem addr); simpl; eauto.
-    + simpl; eauto.
-    + specialize (IHFUEL C st e1 (Config C st (e_app e1 e2) :: l)) as IH.
-      destruct IH as [IH IH'].
-      destruct (eval C st e1 (Config C st (e_app e1 e2) :: l) FUEL);
-      assert (In (Config C st (e_app e1 e2)) reached); try apply IH'; simpl; eauto.
-      destruct v; simpl; eauto.
-      destruct ev as [x e C']. clear IH IH'.
-      specialize (IHFUEL C st0 e2 reached) as IH.
-      destruct IH as [IH IH'].
-      destruct (eval C st0 e2 reached FUEL); eauto.
-      destruct v; eauto. destruct st1.
-      assert (In (Config C st (e_app e1 e2)) reached0); eauto. clear IH IH'.
-      specialize (IHFUEL (C' [|dy_binde x t ([||])|]) (ST (t !-> ev; mem) (tick C (ST mem t) x ev)) e reached0) as IH.
-      destruct IH as [IH IH'].
-      destruct (eval (C' [|dy_binde x t ([||])|])
-                (ST (t !-> ev; mem) (tick C (ST mem t) x ev)) e reached0
-                FUEL); eauto.
-      destruct v; eauto.
-    + specialize (IHFUEL C st e1 (Config C st (e_link e1 e2) :: l)) as IH.
-      destruct IH as [IH IH'].
-      destruct (eval C st e1 (Config C st (e_link e1 e2) :: l) FUEL);
-      assert (In (Config C st (e_link e1 e2)) reached); try apply IH'; simpl; eauto.
-      destruct v; simpl; eauto. clear IH IH'.
-      specialize (IHFUEL mv st0 e2 reached) as IH.
-      destruct IH as [IH IH'].
-      destruct (eval mv st0 e2 reached FUEL); eauto.
-    + simpl. eauto.
-    + destruct (ctx_M C M); simpl; eauto.
-    + specialize (IHFUEL C st e1 (Config C st (m_lete x e1 e2) :: l)) as IH.
-      destruct IH as [IH IH'].
-      destruct (eval C st e1 (Config C st (m_lete x e1 e2) :: l) FUEL);
-      assert (In (Config C st (m_lete x e1 e2)) reached); try apply IH'; simpl; eauto.
-      destruct v; simpl; eauto. destruct st0. clear IH IH'.
-      specialize (IHFUEL (C [|dy_binde x t ([||])|]) (ST (t !-> ev; mem) (tick C (ST mem t) x ev)) e2 reached) as IH.
-      destruct IH as [IH IH'].
-      destruct (eval (C [|dy_binde x t ([||])|])
-                     (ST (t !-> ev; mem) (tick C (ST mem t) x ev)) e2 reached
-                     FUEL); eauto.
-      destruct v; eauto.
-    + specialize (IHFUEL C st e1 (Config C st (m_letm M e1 e2) :: l)) as IH.
-      destruct IH as [IH IH'].
-      destruct (eval C st e1 (Config C st (m_letm M e1 e2) :: l) FUEL);
-      assert (In (Config C st (m_letm M e1 e2)) reached); try apply IH'; simpl; eauto.
-      destruct v; simpl; eauto. clear IH IH'.
-      specialize (IHFUEL (C [|dy_bindm M mv ([||])|]) st0 e2 reached) as IH.
-      destruct IH as [IH IH'].
-      destruct (eval (C [|dy_bindm M mv ([||])|]) st0 e2 reached FUEL); eauto.
-      destruct v; eauto.
-  - intros. destruct e; simpl; eauto.
-    + destruct (addr_x C x); simpl; eauto. destruct st. destruct (mem t); simpl; eauto.
-    + specialize (IHFUEL C st e1 (Config C st (e_app e1 e2) :: l)) as IH.
-      destruct IH as [IH IH'].
-      destruct (eval C st e1 (Config C st (e_app e1 e2) :: l) FUEL);
-      assert (In cf reached); simpl in *; eauto.
-      destruct v; simpl; eauto.
-      destruct ev as [x e C']. clear IH IH'.
-      specialize (IHFUEL C st0 e2 reached) as IH.
-      destruct IH as [IH IH'].
-      destruct (eval C st0 e2 reached FUEL); eauto.
-      destruct v; eauto. destruct st1.
-      assert (In cf reached0); simpl in *; eauto. clear IH IH'.
-      specialize (IHFUEL (C' [|dy_binde x t ([||])|]) (ST (t !-> ev; mem) (tick C (ST mem t) x ev)) e reached0) as IH.
-      destruct IH as [IH IH'].
-      destruct (eval (C' [|dy_binde x t ([||])|])
-                (ST (t !-> ev; mem) (tick C (ST mem t) x ev)) e reached0
-                FUEL); eauto.
-      destruct v; eauto.
-    + specialize (IHFUEL C st e1 (Config C st (e_link e1 e2) :: l)) as IH.
-      destruct IH as [IH IH'].
-      destruct (eval C st e1 (Config C st (e_link e1 e2) :: l) FUEL);
-      assert (In cf reached); try apply IH'; simpl; eauto.
-      destruct v; simpl; eauto. clear IH IH'.
-      specialize (IHFUEL mv st0 e2 reached) as IH.
-      destruct IH as [IH IH'].
-      destruct (eval mv st0 e2 reached FUEL); eauto.
-    + destruct (ctx_M C M); simpl; eauto.
-    + specialize (IHFUEL C st e1 (Config C st (m_lete x e1 e2) :: l)) as IH.
-      destruct IH as [IH IH'].
-      destruct (eval C st e1 (Config C st (m_lete x e1 e2) :: l) FUEL);
-      assert (In cf reached); try apply IH'; simpl; eauto.
-      destruct v; simpl; eauto. destruct st0. clear IH IH'.
-      specialize (IHFUEL (C [|dy_binde x t ([||])|]) (ST (t !-> ev; mem) (tick C (ST mem t) x ev)) e2 reached) as IH.
-      destruct IH as [IH IH'].
-      destruct (eval (C [|dy_binde x t ([||])|])
-                     (ST (t !-> ev; mem) (tick C (ST mem t) x ev)) e2 reached
-                     FUEL); eauto.
-      destruct v; eauto.
-    + specialize (IHFUEL C st e1 (Config C st (m_letm M e1 e2) :: l)) as IH.
-      destruct IH as [IH IH'].
-      destruct (eval C st e1 (Config C st (m_letm M e1 e2) :: l) FUEL);
-      assert (In cf reached); try apply IH'; simpl; eauto.
-      destruct v; simpl; eauto. clear IH IH'.
-      specialize (IHFUEL (C [|dy_bindm M mv ([||])|]) st0 e2 reached) as IH.
-      destruct IH as [IH IH'].
-      destruct (eval (C [|dy_bindm M mv ([||])|]) st0 e2 reached FUEL); eauto.
-      destruct v; eauto.
+  rename H into ET. rename H0 into OT. rename H1 into TT.
+  induction FUEL; intros; try (simpl; eauto; fail).
+  simpl. destruct e; repeat des_goal; simpl; eauto;
+  try rep_with_rew reached1 IHFUEL;
+  try rep_with_rew reached0 IHFUEL;
+  try rep_with_rew reached IHFUEL.
 Qed.
 
-Lemma relax_fuel_reach :
-  forall `{TIME : time T} (C : @dy_ctx T) st e l cf FUEL FUEL' (LE : FUEL <= FUEL'),
-    In cf (extract_reached (eval C st e l FUEL)) ->
-    In cf (extract_reached (eval C st e l FUEL')).
+Ltac clar_eval := 
+  match goal with
+  | [H : eval ?e ?C ?m ?t ?l _ = Error _ |- 
+      context [eval ?e ?C ?m ?t ?l _]] =>
+    rep_eval relax_fuel_err; eauto
+  | [H : eval ?e ?C ?m ?t ?l _ = Resolved _ _ _ _ |-
+      context [eval ?e ?C ?m ?t ?l _]] =>
+    rep_eval relax_fuel; eauto
+  | _ => fail
+  end.
+
+Lemma relax_fuel_reach `{time T} :
+  forall FUEL FUEL' (LE : FUEL <= FUEL') e (C : @dy_ctx T) m t l cf,
+    In cf (extract_reached (eval e C m t l FUEL)) ->
+    In cf (extract_reached (eval e C m t l FUEL')).
 Proof.
-  intros. rename H into H'. rename H0 into H''. rename H1 into H.
-  revert C st e l FUEL' LE H.
+  rename H into ET. rename H0 into OT. rename H1 into TT.
   induction FUEL; intros.
-  - pose proof (reach_myself C st e l FUEL') as [HINT HINT'].
-    inversion H; eauto. rewrite <- H0; eauto.
-  - simpl in H; destruct e; inversion LE; eauto; assert (FUEL <= m) as LE'; try nia.
-    + specialize (IHFUEL C st e1 (Config C st (e_app e1 e2) :: l) m LE') as HINT.
-      destruct (eval C st e1 (Config C st (e_app e1 e2) :: l) FUEL) eqn:EVAL1; simpl;
-      destruct (eval C st e1 (Config C st (e_app e1 e2) :: l) m) eqn:EVAL1'; eauto;
-      try (
-        assert (In cf (extract_reached (eval C st0 e2 reached0 m))) as HINT';
-        try (apply reach_myself; apply HINT; eauto);
-        destruct v; eauto; destruct ev;
-        destruct (eval C st0 e2 reached0 m); eauto;
-        destruct v; eauto; destruct st1;
-        assert (In cf (extract_reached (eval (C0 [|dy_binde x t ([||])|])
-                                             (ST (t !-> ev; mem) (tick C (ST mem t) x ev)) e
-                                             reached1 m))) as HINT'';
-        try (apply reach_myself; apply HINT');
-        destruct (eval (C0 [|dy_binde x t ([||])|])
-                       (ST (t !-> ev; mem) (tick C (ST mem t) x ev)) e
-                       reached1 m); eauto; destruct v; eauto; fail);
-      pose proof (relax_fuel C st e1 (Config C st (e_app e1 e2) :: l) reached v st0 FUEL m LE' EVAL1) as RR;
-      rewrite RR in EVAL1'; inversion EVAL1'; subst.
-      destruct v0; eauto. destruct ev.
-      specialize (IHFUEL C st1 e2 reached0 m LE') as HINT'.
-      destruct (eval C st1 e2 reached0 FUEL) eqn:EVAL2;
-      destruct (eval C st1 e2 reached0 m) eqn:EVAL2'; eauto;
-      try (
-        specialize (HINT' H); destruct v; eauto; destruct st0;
-        assert (In cf (extract_reached (eval (C0 [|dy_binde x t ([||])|])
-                                           (ST (t !-> ev; mem) (tick C (ST mem t) x ev)) e
-                                           reached1 m))) as HINT'';
-        try (apply reach_myself; apply HINT');
-        destruct (eval (C0 [|dy_binde x t ([||])|])
-                       (ST (t !-> ev; mem) (tick C (ST mem t) x ev)) e
-                       reached1 m); eauto; destruct v; eauto);
-      pose proof (relax_fuel C st1 e2 reached0 reached v st0 FUEL m LE' EVAL2) as RR';
-      rewrite RR' in EVAL2'; inversion EVAL2'; subst.
-      destruct v0; eauto. destruct st2.
-      specialize (IHFUEL (C0 [|dy_binde x t ([||])|])
-                         (ST (t !-> ev; mem) (tick C (ST mem t) x ev)) e
-                         reached1 m LE') as HINT''.
-      destruct (eval (C0 [|dy_binde x t ([||])|])
-                     (ST (t !-> ev; mem) (tick C (ST mem t) x ev)) e
-                     reached1 FUEL) eqn:EVAL3;
-      destruct (eval (C0 [|dy_binde x t ([||])|])
-                     (ST (t !-> ev; mem) (tick C (ST mem t) x ev)) e
-                     reached1 m) eqn:EVAL3'; eauto;
-      try (destruct v; eauto); destruct v0; eauto.
-    + specialize (IHFUEL C st e1 (Config C st (e_link e1 e2) :: l) m LE') as HINT.
-      destruct (eval C st e1 (Config C st (e_link e1 e2) :: l) FUEL) eqn:EVAL1; simpl;
-      destruct (eval C st e1 (Config C st (e_link e1 e2) :: l) m) eqn:EVAL1'; eauto;
-      try (
-        destruct v; eauto;
-        assert (In cf (extract_reached (eval mv st0 e2 reached0 m))) as HINT';
-        try (apply reach_myself; apply HINT; eauto);
-        destruct (eval mv st0 e2 reached0 m); eauto; fail);
-      pose proof (relax_fuel C st e1 (Config C st (e_link e1 e2) :: l) reached v st0 FUEL m LE' EVAL1) as RR;
-      rewrite RR in EVAL1'; inversion EVAL1'; subst.
-      destruct v0; eauto.
-      destruct (eval mv st1 e2 reached0 FUEL) eqn:EVAL2; simpl;
-      destruct (eval mv st1 e2 reached0 m) eqn:EVAL2';
-      try (
-        assert (In cf (extract_reached (eval mv st1 e2 reached0 m))) as HINT';
-        try (apply IHFUEL; eauto; rewrite EVAL2; eauto);
-        rewrite EVAL2' in HINT'; eauto).
-    + specialize (IHFUEL C st e1 (Config C st (m_lete x e1 e2) :: l) m LE') as HINT.
-      destruct (eval C st e1 (Config C st (m_lete x e1 e2) :: l) FUEL) eqn:EVAL1; simpl;
-      destruct (eval C st e1 (Config C st (m_lete x e1 e2) :: l) m) eqn:EVAL1'; eauto;
-      try (
-        destruct v; eauto; destruct st0;
-        assert (In cf (extract_reached (eval (C [|dy_binde x t ([||])|])
-                                             (ST (t !-> ev; mem) (tick C (ST mem t) x ev)) e2
-                                             reached0 m))) as HINT';
-        try (apply reach_myself; apply HINT; eauto);
-        destruct (eval (C [|dy_binde x t ([||])|])
-                       (ST (t !-> ev; mem) (tick C (ST mem t) x ev)) e2
-                       reached0 m); eauto; destruct v; eauto; fail);
-      pose proof (relax_fuel C st e1 (Config C st (m_lete x e1 e2) :: l) reached v st0 FUEL m LE' EVAL1) as RR;
-      rewrite RR in EVAL1'; inversion EVAL1'; subst.
-      destruct v0; eauto. destruct st1.
-      destruct (eval (C [|dy_binde x t ([||])|])
-                     (ST (t !-> ev; mem) (tick C (ST mem t) x ev)) e2 reached0
-                     FUEL) eqn:EVAL2; simpl;
-      destruct (eval (C [|dy_binde x t ([||])|])
-                     (ST (t !-> ev; mem) (tick C (ST mem t) x ev)) e2 reached0
-                     m) eqn:EVAL2';
-      try (
-        assert (In cf (extract_reached (eval (C [|dy_binde x t ([||])|])
-                                             (ST (t !-> ev; mem) (tick C (ST mem t) x ev)) e2 reached0
-                                             m))) as HINT';
-        try (apply IHFUEL; eauto; rewrite EVAL2; eauto);
-        rewrite EVAL2' in HINT'; eauto; destruct v; eauto);
-      pose proof (relax_fuel (C [|dy_binde x t ([||])|])
-                             (ST (t !-> ev; mem) (tick C (ST mem t) x ev)) e2
-                             reached0 reached v st0 FUEL m LE' EVAL2) as RR';
-      rewrite RR' in EVAL2'; inversion EVAL2'; subst.
-      destruct v0; eauto.
-    + specialize (IHFUEL C st e1 (Config C st (m_letm M e1 e2) :: l) m LE') as HINT.
-      destruct (eval C st e1 (Config C st (m_letm M e1 e2) :: l) FUEL) eqn:EVAL1; simpl;
-      destruct (eval C st e1 (Config C st (m_letm M e1 e2) :: l) m) eqn:EVAL1'; eauto;
-      try (
-        destruct v; eauto;
-        assert (In cf (extract_reached (eval (C [|dy_bindm M mv ([||])|]) st0 e2 reached0 m))) as HINT';
-        try (apply reach_myself; apply HINT; eauto);
-        destruct (eval (C [|dy_bindm M mv ([||])|]) st0 e2 reached0 m); eauto; destruct v; eauto; fail);
-      pose proof (relax_fuel C st e1 (Config C st (m_letm M e1 e2) :: l) reached v st0 FUEL m LE' EVAL1) as RR;
-      rewrite RR in EVAL1'; inversion EVAL1'; subst.
-      destruct v0; eauto.
-      destruct (eval (C [|dy_bindm M mv ([||])|]) st1 e2 reached0 FUEL) eqn:EVAL2; simpl;
-      destruct (eval (C [|dy_bindm M mv ([||])|]) st1 e2 reached0 m) eqn:EVAL2';
-      try (
-        assert (In cf (extract_reached (eval (C [|dy_bindm M mv ([||])|]) st1 e2 reached0 m))) as HINT';
-        try (apply IHFUEL; eauto; rewrite EVAL2; eauto);
-        rewrite EVAL2' in HINT'; eauto; destruct v; eauto; fail);
-      pose proof (relax_fuel (C [|dy_bindm M mv ([||])|]) st1 e2 reached0 reached v st0 FUEL m LE' EVAL2) as RR';
-      rewrite RR' in EVAL2'; inversion EVAL2'; subst.
-      destruct v0; eauto.
+  simpl in *. apply reach_myself. eauto.
+  inversion LE; subst. assumption.
+  assert (FUEL <= m0) as HINT. { nia. }
+  destruct e; simpl in *; eauto.
+  - des_hyp; try clar_eval.
+    repeat des_goal;
+    try rep_with_rew reached2 reach_myself;
+    try rep_with_rew reached1 reach_myself;
+    try rep_with_rew reached0 IHFUEL;
+    try rep_eval idtac; eauto.
+    des_hyp; simpl; eauto.
+    des_hyp. des_hyp; try clar_eval.
+    repeat des_goal;
+    try rep_with_rew reached2 reach_myself;
+    try rep_with_rew reached1 IHFUEL;
+    try rep_eval idtac; eauto.
+    des_hyp; simpl; eauto.
+    des_hyp; try clar_eval.
+    repeat des_goal;
+    try rep_with_rew reached2 IHFUEL;
+    rep_eval idtac; eauto.
+  - des_hyp; try clar_eval.
+    repeat des_goal;
+    try rep_with_rew reached1 reach_myself;
+    try rep_with_rew reached0 IHFUEL;
+    try rep_eval idtac; eauto.
+    des_hyp; simpl; eauto.
+    des_hyp; try clar_eval.
+    repeat des_goal;
+    try rep_with_rew reached1 IHFUEL;
+    rep_eval idtac; eauto.
+  - des_hyp; try clar_eval.
+    repeat des_goal;
+    try rep_with_rew reached1 reach_myself;
+    try rep_with_rew reached0 IHFUEL;
+    try rep_eval idtac; eauto.
+    des_hyp; simpl; eauto.
+    des_hyp; try clar_eval.
+    repeat des_goal;
+    try rep_with_rew reached1 IHFUEL;
+    rep_eval idtac; eauto.
+  - des_hyp; try clar_eval.
+    repeat des_goal;
+    try rep_with_rew reached1 reach_myself;
+    try rep_with_rew reached0 IHFUEL;
+    try rep_eval idtac; eauto.
+    des_hyp; simpl; eauto.
+    des_hyp; try clar_eval.
+    repeat des_goal;
+    try rep_with_rew reached1 IHFUEL;
+    rep_eval idtac; eauto.
 Qed.
 
-Lemma reach_same :
-  forall `{TIME : time T} FUEL (C : @dy_ctx T) st e l l'
-          (CONTAINED : forall cf, In cf l -> In cf l'),
-    match (eval C st e l FUEL), (eval C st e l' FUEL) with
-    | Resolved v st_v reached, Resolved v' st_v' reached' => 
-      v = v' /\ st_v = st_v' /\ (forall cf, In cf reached -> In cf reached')
+Lemma reach_same `{time T} :
+  forall FUEL e (C : @dy_ctx T) m t l l'
+        (CONTAINED : forall cf, In cf l -> In cf l'),
+    match (eval e C m t l FUEL), (eval e C m t l' FUEL) with
+    | Resolved V m t reached, Resolved V' m' t' reached' => 
+      V = V' /\ m = m' /\ t = t' /\ (forall cf, In cf reached -> In cf reached')
     | Error reached, Error reached'
     | Pending reached, Pending reached' =>
       forall cf, In cf reached -> In cf reached'
     | _, _ => False
     end.
 Proof.
-  intros. rename H into ET. rename H0 into OT.
-  revert C st e l l' CONTAINED. induction FUEL; intros.
+  rename H into ET. rename H0 into OT. rename H1 into TT.
+  induction FUEL; intros.
   simpl. intros. destruct H; eauto.
-  destruct e; simpl; eauto.
-  - destruct (addr_x C x); destruct st; destruct (mem t); repeat split; intros; destruct H; simpl; eauto.
-  - repeat split; intros; destruct H; eauto.
-  - assert ((forall cf : config,
-                    In cf (Config C st (e_app e1 e2) :: l) ->
-                    In cf (Config C st (e_app e1 e2) :: l'))) as CONTAINED'.
-    { intros. simpl in *. destruct H; eauto. }
-    specialize (IHFUEL C st e1 (Config C st (e_app e1 e2) :: l) (Config C st (e_app e1 e2) :: l') CONTAINED') as IHl.
-    clear CONTAINED'.
-    destruct (eval C st e1 (Config C st (e_app e1 e2) :: l) FUEL);
-    destruct (eval C st e1 (Config C st (e_app e1 e2) :: l') FUEL);
-    try (assert False as contra; eauto; inversion contra); eauto.
-    destruct IHl as [RR [RR' CONTAINED']]. rewrite <- RR in *. rewrite <- RR' in *. clear RR RR'.
-    destruct v; eauto. destruct ev.
-    specialize (IHFUEL C st0 e2 reached reached0 CONTAINED') as IHr.
-    clear CONTAINED'.
-    destruct (eval C st0 e2 reached FUEL);
-    destruct (eval C st0 e2 reached0 FUEL);
-    try (assert False as contra; eauto; inversion contra); eauto.
-    destruct IHr as [RR [RR' CONTAINED']]. rewrite <- RR in *. rewrite <- RR' in *. clear RR RR'.
-    destruct v; eauto. destruct st2.
-    specialize (IHFUEL (C0 [|dy_binde x t ([||])|])
-                       (ST (t !-> ev; mem) (tick C (ST mem t) x ev))
-                       e reached1 reached2 CONTAINED').
-    clear CONTAINED'.
-    destruct (eval (C0 [|dy_binde x t ([||])|])
-                   (ST (t !-> ev; mem) (tick C (ST mem t) x ev))
-                   e reached1 FUEL);
-    destruct (eval (C0 [|dy_binde x t ([||])|])
-                   (ST (t !-> ev; mem) (tick C (ST mem t) x ev))
-                   e reached2 FUEL);
-    try (assert False as contra; eauto; inversion contra); eauto.
-    destruct IHFUEL as [RR [RR' CONTAINED']]. rewrite <- RR in *. rewrite <- RR' in *. clear RR RR'.
-    destruct v; eauto.
-  - assert ((forall cf : config,
-                    In cf (Config C st (e_link e1 e2) :: l) ->
-                    In cf (Config C st (e_link e1 e2) :: l'))) as CONTAINED'.
-    { intros. simpl in *. destruct H; eauto. }
-    specialize (IHFUEL C st e1 (Config C st (e_link e1 e2) :: l) (Config C st (e_link e1 e2) :: l') CONTAINED') as IHl.
-    clear CONTAINED'.
-    destruct (eval C st e1 (Config C st (e_link e1 e2) :: l) FUEL);
-    destruct (eval C st e1 (Config C st (e_link e1 e2) :: l') FUEL);
-    try (assert False as contra; eauto; inversion contra); eauto.
-    destruct IHl as [RR [RR' CONTAINED']]. rewrite <- RR in *. rewrite <- RR' in *. clear RR RR'.
-    destruct v; eauto.
-    specialize (IHFUEL mv st0 e2 reached reached0 CONTAINED') as IHr. clear CONTAINED'.
-    destruct (eval mv st0 e2 reached FUEL);
-    destruct (eval mv st0 e2 reached0 FUEL);
-    try (assert False as contra; eauto; inversion contra); eauto.
-  - repeat split; eauto. intros; destruct H; eauto.
-  - destruct (ctx_M C M); eauto; repeat split; intros; simpl in *; destruct H; eauto.
-  - assert ((forall cf : config,
-                    In cf (Config C st (m_lete x e1 e2) :: l) ->
-                    In cf (Config C st (m_lete x e1 e2) :: l'))) as CONTAINED'.
-    { intros. simpl in *. destruct H; eauto. }
-    specialize (IHFUEL C st e1 (Config C st (m_lete x e1 e2) :: l) (Config C st (m_lete x e1 e2) :: l') CONTAINED') as IHl.
-    clear CONTAINED'.
-    destruct (eval C st e1 (Config C st (m_lete x e1 e2) :: l) FUEL);
-    destruct (eval C st e1 (Config C st (m_lete x e1 e2) :: l') FUEL);
-    try (assert False as contra; eauto; inversion contra); eauto.
-    destruct IHl as [RR [RR' CONTAINED']]. rewrite <- RR in *. rewrite <- RR' in *. clear RR RR'.
-    destruct v; eauto. destruct st0.
-    specialize (IHFUEL (C [|dy_binde x t ([||])|])
-                       (ST (t !-> ev; mem) (tick C (ST mem t) x ev))
-                       e2 reached reached0 CONTAINED'). clear CONTAINED'.
-    destruct (eval (C [|dy_binde x t ([||])|])
-                   (ST (t !-> ev; mem) (tick C (ST mem t) x ev))
-                   e2 reached FUEL);
-    destruct (eval (C [|dy_binde x t ([||])|])
-                   (ST (t !-> ev; mem) (tick C (ST mem t) x ev))
-                   e2 reached0 FUEL);
-    try (assert False as contra; eauto; inversion contra); eauto.
-    destruct IHFUEL as [RR [RR' CONTAINED']]. rewrite <- RR in *. rewrite <- RR' in *.
-    destruct v; eauto.
-  - assert ((forall cf : config,
-                    In cf (Config C st (m_letm M e1 e2) :: l) ->
-                    In cf (Config C st (m_letm M e1 e2) :: l'))) as CONTAINED'.
-    { intros. simpl in *. destruct H; eauto. }
-    specialize (IHFUEL C st e1 (Config C st (m_letm M e1 e2) :: l) (Config C st (m_letm M e1 e2) :: l') CONTAINED') as IHl.
-    clear CONTAINED'.
-    destruct (eval C st e1 (Config C st (m_letm M e1 e2) :: l) FUEL);
-    destruct (eval C st e1 (Config C st (m_letm M e1 e2) :: l') FUEL);
-    try (assert False as contra; eauto; inversion contra); eauto.
-    destruct IHl as [RR [RR' CONTAINED']]. rewrite <- RR in *. rewrite <- RR' in *. clear RR RR'.
-    destruct v; eauto.
-    specialize (IHFUEL (C [|dy_bindm M mv ([||])|]) st0 e2 reached reached0 CONTAINED'). clear CONTAINED'.
-    destruct (eval (C [|dy_bindm M mv ([||])|]) st0 e2 reached FUEL);
-    destruct (eval (C [|dy_bindm M mv ([||])|]) st0 e2 reached0 FUEL);
-    try (assert False as contra; eauto; inversion contra); eauto.
-    destruct IHFUEL as [RR [RR' CONTAINED']]. rewrite <- RR in *. rewrite <- RR' in *.
-    destruct v; eauto.
+  assert ((forall cf : config,
+            In cf (Cf e C m t :: l) ->
+            In cf (Cf e C m t :: l'))) as CONTAINED'.
+  { intros. simpl in *. destruct H; eauto. }
+  destruct e; simpl; eauto;
+  try (
+    (* trivial cases *)
+    lazymatch goal with 
+    | |- context [eval _ _ _ _ _ _] => fail
+    | _ => idtac
+    end;
+    repeat des_goal; repeat des_hyp; clarify;
+    repeat split; eauto;
+    intros cf OR; simpl in *; destruct OR; eauto);
+  match goal with
+    | |- context [eval ?e ?C ?m ?t _ _] =>
+      specialize (IHFUEL e C m t _ _ CONTAINED') as CONTAINED''
+    | _ => fail
+  end;
+  repeat des_hyp; eauto;
+  destruct CONTAINED'' as [? [? [? CONTAINED'']]]; subst;
+  des_goal; repeat des_hyp; clarify;
+  match goal with
+  | |- context [eval ?e ?C ?m ?t _ _] =>
+    specialize (IHFUEL e C m t _ _ CONTAINED'') as CONTAINED'''
+  | _ => fail
+  end;
+  repeat des_hyp; clarify;
+  destruct CONTAINED''' as [? [? [? CONTAINED''']]]; subst; eauto;
+  match goal with
+  | |- context [eval ?e ?C ?m ?t _ _] =>
+    specialize (IHFUEL e C m t _ _ CONTAINED''') as CONTAINED''''
+  | _ => fail
+  end;
+  repeat des_hyp; clarify;
+  destruct CONTAINED'''' as [? [? [? ?]]]; clarify.
 Qed.
 
-Lemma separate_reach :
-  forall `{TIME : time T} FUEL (C : @dy_ctx T) st e l cf,
-    In cf (extract_reached (eval C st e l FUEL)) <->
-    In cf l \/ In cf (extract_reached (eval C st e [] FUEL)).
+Ltac separate_reach_tac cf IHFUEL HINT HINT' RR RR' :=
+  match goal with
+  | [H : context [match eval ?e ?C ?m ?t ?l ?n with _ => _ end] |-
+      context [match eval ?e ?C ?m ?t ?l0 ?n with _ => _ end]] =>
+    specialize (IHFUEL e C m t l cf) as HINT;
+    specialize (IHFUEL e C m t l0 cf) as HINT';
+    pose proof (reach_same n e C m t l0 l RR) as RR';
+    clear RR
+  | [H : context [match eval ?e ?C ?m ?t ?l ?n with _ => _ end] |-
+      context [match eval ?e ?C ?m ?t ?l0 ?n with _ => _ end]] =>
+    specialize (IHFUEL e C m t l cf) as HINT;
+    specialize (IHFUEL e C m t l0 cf) as HINT';
+    pose proof (reach_same n e C m t l l0 RR) as RR';
+    clear RR
+  | _ => fail
+  end.
+
+Lemma separate_reach `{time T} :
+  forall FUEL e (C : @dy_ctx T) m t l cf,
+    In cf (extract_reached (eval e C m t l FUEL)) <->
+    In cf l \/ In cf (extract_reached (eval e C m t [] FUEL)).
 Proof.
-  intros. rename H into ET. rename H0 into OT.
-  revert C st e l cf. induction FUEL; intros; simpl; split; intros.
-  - destruct H; eauto. 
-  - destruct H as [?|[?|?]]; eauto. exfalso; eauto.
-  - destruct e.
-    + destruct (addr_x C x); destruct st; destruct (mem t); simpl in *;
-      destruct H; eauto.
-    + simpl in *; destruct H; eauto.
-    + specialize (IHFUEL C st e1 (Config C st (e_app e1 e2) :: l) cf) as HINT1.
-      specialize (IHFUEL C st e1 [Config C st (e_app e1 e2)] cf) as HINT1'.
-      assert (forall cf, In cf [Config C st (e_app e1 e2)] ->
-                         In cf (Config C st (e_app e1 e2) :: l)) as CONTAINED.
-      { intros; simpl in *; destruct H0; eauto. inversion H0. }
-      pose proof (reach_same FUEL C st e1 [Config C st (e_app e1 e2)] (Config C st (e_app e1 e2) :: l) CONTAINED) as contra.
-      clear CONTAINED.
-      destruct (eval C st e1 (Config C st (e_app e1 e2) :: l) FUEL);
-      destruct (eval C st e1 [Config C st (e_app e1 e2)] FUEL);
-      try (rewrite HINT1 in H); try rewrite HINT1';
-      try (simpl in *; destruct H as [[?|?]|?]; eauto; fail);
-      try (inversion contra; fail).
-      destruct contra as [RR [RR' CONTAINED]]. rewrite RR in *. rewrite RR' in *. clear RR RR'.
-      destruct v;
-      try (rewrite HINT1 in H; rewrite HINT1'; destruct H as [[?|?]|?]; simpl in *; eauto).
-      destruct ev. simpl in *.
-      specialize (IHFUEL C st0 e2 reached cf) as HINT2.
-      specialize (IHFUEL C st0 e2 reached0 cf) as HINT2'.
-      pose proof (reach_same FUEL C st0 e2 reached0 reached CONTAINED) as contra.
-      clear CONTAINED.
-      destruct (eval C st0 e2 reached FUEL);
-      destruct (eval C st0 e2 reached0 FUEL);
-      try (rewrite HINT2 in H); try rewrite HINT2';
-      try (rewrite HINT1 in H); try rewrite HINT1';
-      try (simpl in *; destruct H as [[[?|?]|?]|?]; eauto; fail);
-      try (inversion contra; fail).
-      destruct contra as [RR [RR' CONTAINED]]. rewrite RR in *. rewrite RR' in *. clear RR RR'.
-      destruct v;
-      try (rewrite HINT2 in H; rewrite HINT2'; rewrite HINT1 in H; rewrite HINT1';
-          destruct H as [[[?|?]|?]|?]; simpl in *; eauto).
-      destruct st2.
-      specialize (IHFUEL (C0 [|dy_binde x t ([||])|])
-                         (ST (t !-> ev; mem) (tick C (ST mem t) x ev)) 
-                         e reached1 cf) as HINT3.
-      specialize (IHFUEL (C0 [|dy_binde x t ([||])|])
-                         (ST (t !-> ev; mem) (tick C (ST mem t) x ev)) 
-                         e reached2 cf) as HINT3'.
-      pose proof (reach_same FUEL (C0 [|dy_binde x t ([||])|])
-                                  (ST (t !-> ev; mem) (tick C (ST mem t) x ev))
-                                  e reached2 reached1 CONTAINED) as contra. clear CONTAINED.
-      destruct (eval (C0 [|dy_binde x t ([||])|])
-                     (ST (t !-> ev; mem) (tick C (ST mem t) x ev)) e
-                     reached1 FUEL);
-      destruct (eval (C0 [|dy_binde x t ([||])|])
-                     (ST (t !-> ev; mem) (tick C (ST mem t) x ev)) e
-                     reached2 FUEL);
-      try (rewrite HINT3 in H); try rewrite HINT3';
-      try (rewrite HINT2 in H); try rewrite HINT2';
-      try (rewrite HINT1 in H); try rewrite HINT1';
-      try (simpl in *; destruct H as [[[[?|?]|?]|?]|?]; eauto 7; fail);
-      try (inversion contra; fail).
-      destruct contra as [RR [RR' CONTAINED]]. rewrite RR in *. rewrite RR' in *. clear RR RR'.
-      destruct v; simpl in *;
-      rewrite HINT3 in H; rewrite HINT3';
-      rewrite HINT2 in H; rewrite HINT2';
-      rewrite HINT1 in H; rewrite HINT1';
-      destruct H as [[[[?|?]|?]|?]|?]; eauto 7.
-    + specialize (IHFUEL C st e1 (Config C st (e_link e1 e2) :: l) cf) as HINT1.
-      specialize (IHFUEL C st e1 [Config C st (e_link e1 e2)] cf) as HINT1'.
-      assert (forall cf, In cf [Config C st (e_link e1 e2)] ->
-                         In cf (Config C st (e_link e1 e2) :: l)) as CONTAINED.
-      { intros; simpl in *; destruct H0; eauto. inversion H0. }
-      pose proof (reach_same FUEL C st e1 [Config C st (e_link e1 e2)] (Config C st (e_link e1 e2) :: l) CONTAINED) as contra.
-      clear CONTAINED.
-      destruct (eval C st e1 (Config C st (e_link e1 e2) :: l) FUEL);
-      destruct (eval C st e1 [Config C st (e_link e1 e2)] FUEL);
-      try (rewrite HINT1 in H); try rewrite HINT1';
-      try (simpl in *; destruct H as [[?|?]|?]; eauto; fail);
-      try (inversion contra; fail).
-      destruct contra as [RR [RR' CONTAINED]]. rewrite RR in *. rewrite RR' in *. clear RR RR'.
-      destruct v;
-      try (rewrite HINT1 in H; rewrite HINT1'; destruct H as [[?|?]|?]; simpl in *; eauto).
-      specialize (IHFUEL mv st0 e2 reached cf) as HINT2.
-      specialize (IHFUEL mv st0 e2 reached0 cf) as HINT2'.
-      pose proof (reach_same FUEL mv st0 e2 reached0 reached CONTAINED) as contra.
-      clear CONTAINED.
-      destruct (eval mv st0 e2 reached FUEL);
-      destruct (eval mv st0 e2 reached0 FUEL);
-      try (rewrite HINT2 in H); try rewrite HINT2';
-      try (rewrite HINT1 in H); try rewrite HINT1';
-      try (simpl in *; destruct H as [[[?|?]|?]|?]; eauto; fail);
-      try (inversion contra; fail).
-    + simpl in *. destruct H; eauto.
-    + destruct (ctx_M C M); simpl in *; destruct H; eauto.
-    + specialize (IHFUEL C st e1 (Config C st (m_lete x e1 e2) :: l) cf) as HINT1.
-      specialize (IHFUEL C st e1 [Config C st (m_lete x e1 e2)] cf) as HINT1'.
-      assert (forall cf, In cf [Config C st (m_lete x e1 e2)] ->
-                         In cf (Config C st (m_lete x e1 e2) :: l)) as CONTAINED.
-      { intros; simpl in *; destruct H0; eauto. inversion H0. }
-      pose proof (reach_same FUEL C st e1 [Config C st (m_lete x e1 e2)] (Config C st (m_lete x e1 e2) :: l) CONTAINED) as contra.
-      clear CONTAINED.
-      destruct (eval C st e1 (Config C st (m_lete x e1 e2) :: l) FUEL);
-      destruct (eval C st e1 [Config C st (m_lete x e1 e2)] FUEL);
-      try (rewrite HINT1 in H); try rewrite HINT1';
-      try (simpl in *; destruct H as [[?|?]|?]; eauto; fail);
-      try (inversion contra; fail).
-      destruct contra as [RR [RR' CONTAINED]]. rewrite RR in *. rewrite RR' in *. clear RR RR'.
-      destruct v;
-      try (rewrite HINT1 in H; rewrite HINT1'; destruct H as [[?|?]|?]; simpl in *; eauto). destruct st0.
-      specialize (IHFUEL (C [|dy_binde x t ([||])|])
-                         (ST (t !-> ev; mem) (tick C (ST mem t) x ev))
-                         e2 reached cf) as HINT2.
-      specialize (IHFUEL (C [|dy_binde x t ([||])|])
-                         (ST (t !-> ev; mem) (tick C (ST mem t) x ev))
-                         e2 reached0 cf) as HINT2'.
-      pose proof (reach_same FUEL (C [|dy_binde x t ([||])|])
-                                  (ST (t !-> ev; mem) (tick C (ST mem t) x ev))
-                                  e2 reached0 reached CONTAINED) as contra.
-      clear CONTAINED.
-      destruct (eval (C [|dy_binde x t ([||])|])
-                     (ST (t !-> ev; mem) (tick C (ST mem t) x ev))
-                     e2 reached FUEL);
-      destruct (eval (C [|dy_binde x t ([||])|])
-                     (ST (t !-> ev; mem) (tick C (ST mem t) x ev))
-                     e2 reached0 FUEL);
-      try (rewrite HINT2 in H); try rewrite HINT2';
-      try (rewrite HINT1 in H); try rewrite HINT1';
-      try (simpl in *; destruct H as [[[?|?]|?]|?]; eauto; fail);
-      try (inversion contra; fail).
-      destruct contra as [RR [RR' CONTAINED]]. rewrite RR in *. rewrite RR' in *. clear RR RR'.
-      destruct v; rewrite HINT2 in H; try rewrite HINT2';
-      rewrite HINT1 in H; try rewrite HINT1';
-      simpl in *; destruct H as [[[?|?]|?]|?]; eauto.
-    + specialize (IHFUEL C st e1 (Config C st (m_letm M e1 e2) :: l) cf) as HINT1.
-      specialize (IHFUEL C st e1 [Config C st (m_letm M e1 e2)] cf) as HINT1'.
-      assert (forall cf, In cf [Config C st (m_letm M e1 e2)] ->
-                         In cf (Config C st (m_letm M e1 e2) :: l)) as CONTAINED.
-      { intros; simpl in *; destruct H0; eauto. inversion H0. }
-      pose proof (reach_same FUEL C st e1 [Config C st (m_letm M e1 e2)] (Config C st (m_letm M e1 e2) :: l) CONTAINED) as contra.
-      clear CONTAINED.
-      destruct (eval C st e1 (Config C st (m_letm M e1 e2) :: l) FUEL);
-      destruct (eval C st e1 [Config C st (m_letm M e1 e2)] FUEL);
-      try (rewrite HINT1 in H); try rewrite HINT1';
-      try (simpl in *; destruct H as [[?|?]|?]; eauto; fail);
-      try (inversion contra; fail).
-      destruct contra as [RR [RR' CONTAINED]]. rewrite RR in *. rewrite RR' in *. clear RR RR'.
-      destruct v;
-      try (rewrite HINT1 in H; rewrite HINT1'; destruct H as [[?|?]|?]; simpl in *; eauto).
-      specialize (IHFUEL (C [|dy_bindm M mv ([||])|]) st0 e2 reached cf) as HINT2.
-      specialize (IHFUEL (C [|dy_bindm M mv ([||])|]) st0 e2 reached0 cf) as HINT2'.
-      pose proof (reach_same FUEL (C [|dy_bindm M mv ([||])|]) st0 e2 reached0 reached CONTAINED) as contra.
-      clear CONTAINED.
-      destruct (eval (C [|dy_bindm M mv ([||])|]) st0 e2 reached FUEL);
-      destruct (eval (C [|dy_bindm M mv ([||])|]) st0 e2 reached0 FUEL);
-      try (rewrite HINT2 in H); try rewrite HINT2';
-      try (rewrite HINT1 in H); try rewrite HINT1';
-      try (simpl in *; destruct H as [[[?|?]|?]|?]; eauto; fail);
-      try (inversion contra; fail).
-      destruct contra as [RR [RR' CONTAINED]]. rewrite RR in *. rewrite RR' in *. clear RR RR'.
-      destruct v; rewrite HINT2 in H; rewrite HINT2';
-      rewrite HINT1 in H; rewrite HINT1';
-      simpl in *; destruct H as [[[?|?]|?]|?]; eauto.
-  - destruct e.
-    + destruct (addr_x C x); destruct st; destruct (mem t); simpl in *; destruct H as [?|[?|?]]; eauto; inversion H.
-    + simpl in *; destruct H as [?|[?|?]]; eauto; inversion H.
-    + specialize (IHFUEL C st e1 (Config C st (e_app e1 e2) :: l) cf) as HINT1'.
-      specialize (IHFUEL C st e1 [Config C st (e_app e1 e2)] cf) as HINT1.
-      assert (forall cf, In cf [Config C st (e_app e1 e2)] ->
-                         In cf (Config C st (e_app e1 e2) :: l)) as CONTAINED.
-      { intros; simpl in *; destruct H0; eauto. inversion H0. }
-      pose proof (reach_same FUEL C st e1 [Config C st (e_app e1 e2)] (Config C st (e_app e1 e2) :: l) CONTAINED) as contra.
-      clear CONTAINED.
-      destruct (eval C st e1 (Config C st (e_app e1 e2) :: l) FUEL);
-      destruct (eval C st e1 [Config C st (e_app e1 e2)] FUEL);
-      try (rewrite HINT1 in H); try rewrite HINT1';
-      try (simpl in *; destruct H as [?|[[?|?]|?]]; eauto; inversion H; fail);
-      try (inversion contra; fail).
-      destruct contra as [RR [RR' CONTAINED]]. rewrite RR in *. rewrite RR' in *. clear RR RR'.
-      destruct v;
-      try (rewrite HINT1 in H; rewrite HINT1'; destruct H as [?|[[?|?]|?]]; simpl in *; eauto; inversion H).
-      destruct ev. simpl in *.
-      specialize (IHFUEL C st0 e2 reached cf) as HINT2'.
-      specialize (IHFUEL C st0 e2 reached0 cf) as HINT2.
-      pose proof (reach_same FUEL C st0 e2 reached0 reached CONTAINED) as contra.
-      clear CONTAINED.
-      destruct (eval C st0 e2 reached FUEL);
-      destruct (eval C st0 e2 reached0 FUEL);
-      try (rewrite HINT2 in H); try rewrite HINT2';
-      try (rewrite HINT1 in H); try rewrite HINT1';
-      try (simpl in *; destruct H as [?|[[[?|?]|?]|?]]; eauto; inversion H; fail);
-      try (inversion contra; fail).
-      destruct contra as [RR [RR' CONTAINED]]. rewrite RR in *. rewrite RR' in *. clear RR RR'.
-      destruct v;
-      try (rewrite HINT2 in H; rewrite HINT2'; rewrite HINT1 in H; rewrite HINT1';
-          destruct H as [?|[[[?|?]|?]|?]]; simpl in *; eauto; inversion H).
-      destruct st2.
-      specialize (IHFUEL (C0 [|dy_binde x t ([||])|])
-                         (ST (t !-> ev; mem) (tick C (ST mem t) x ev)) 
-                         e reached1 cf) as HINT3'.
-      specialize (IHFUEL (C0 [|dy_binde x t ([||])|])
-                         (ST (t !-> ev; mem) (tick C (ST mem t) x ev)) 
-                         e reached2 cf) as HINT3.
-      pose proof (reach_same FUEL (C0 [|dy_binde x t ([||])|])
-                                  (ST (t !-> ev; mem) (tick C (ST mem t) x ev))
-                                  e reached2 reached1 CONTAINED) as contra. clear CONTAINED.
-      destruct (eval (C0 [|dy_binde x t ([||])|])
-                     (ST (t !-> ev; mem) (tick C (ST mem t) x ev)) e
-                     reached1 FUEL);
-      destruct (eval (C0 [|dy_binde x t ([||])|])
-                     (ST (t !-> ev; mem) (tick C (ST mem t) x ev)) e
-                     reached2 FUEL);
-      try (rewrite HINT3 in H); try rewrite HINT3';
-      try (rewrite HINT2 in H); try rewrite HINT2';
-      try (rewrite HINT1 in H); try rewrite HINT1';
-      try (simpl in *; destruct H as [?|[[[[?|?]|?]|?]|?]]; eauto 7; inversion H; fail);
-      try (inversion contra; fail).
-      destruct contra as [RR [RR' CONTAINED]]. rewrite RR in *. rewrite RR' in *. clear RR RR'.
-      destruct v; simpl in *;
-      rewrite HINT3 in H; rewrite HINT3';
-      rewrite HINT2 in H; rewrite HINT2';
-      rewrite HINT1 in H; rewrite HINT1';
-      destruct H as [?|[[[[?|?]|?]|?]|?]]; eauto 7; inversion H.
-    + specialize (IHFUEL C st e1 (Config C st (e_link e1 e2) :: l) cf) as HINT1'.
-      specialize (IHFUEL C st e1 [Config C st (e_link e1 e2)] cf) as HINT1.
-      assert (forall cf, In cf [Config C st (e_link e1 e2)] ->
-                         In cf (Config C st (e_link e1 e2) :: l)) as CONTAINED.
-      { intros; simpl in *; destruct H0; eauto. inversion H0. }
-      pose proof (reach_same FUEL C st e1 [Config C st (e_link e1 e2)] (Config C st (e_link e1 e2) :: l) CONTAINED) as contra.
-      clear CONTAINED.
-      destruct (eval C st e1 (Config C st (e_link e1 e2) :: l) FUEL);
-      destruct (eval C st e1 [Config C st (e_link e1 e2)] FUEL);
-      try (rewrite HINT1 in H); try rewrite HINT1';
-      try (simpl in *; destruct H as [?|[[?|?]|?]]; eauto; inversion H; fail);
-      try (inversion contra; fail).
-      destruct contra as [RR [RR' CONTAINED]]. rewrite RR in *. rewrite RR' in *. clear RR RR'.
-      destruct v;
-      try (rewrite HINT1 in H; rewrite HINT1'; destruct H as [?|[[?|?]|?]]; simpl in *; eauto; inversion H).
-      specialize (IHFUEL mv st0 e2 reached cf) as HINT2'.
-      specialize (IHFUEL mv st0 e2 reached0 cf) as HINT2.
-      pose proof (reach_same FUEL mv st0 e2 reached0 reached CONTAINED) as contra.
-      clear CONTAINED.
-      destruct (eval mv st0 e2 reached FUEL);
-      destruct (eval mv st0 e2 reached0 FUEL);
-      try (rewrite HINT2 in H); try rewrite HINT2';
-      try (rewrite HINT1 in H); try rewrite HINT1';
-      try (simpl in *; destruct H as [?|[[[?|?]|?]|?]]; eauto; inversion H; fail);
-      try (inversion contra; fail).
-    + simpl in *. destruct H as [?|[?|?]]; eauto; inversion H.
-    + destruct (ctx_M C M); simpl in *; destruct H as [?|[?|?]]; eauto; inversion H.
-    + specialize (IHFUEL C st e1 (Config C st (m_lete x e1 e2) :: l) cf) as HINT1'.
-      specialize (IHFUEL C st e1 [Config C st (m_lete x e1 e2)] cf) as HINT1.
-      assert (forall cf, In cf [Config C st (m_lete x e1 e2)] ->
-                         In cf (Config C st (m_lete x e1 e2) :: l)) as CONTAINED.
-      { intros; simpl in *; destruct H0; eauto. inversion H0. }
-      pose proof (reach_same FUEL C st e1 [Config C st (m_lete x e1 e2)] (Config C st (m_lete x e1 e2) :: l) CONTAINED) as contra.
-      clear CONTAINED.
-      destruct (eval C st e1 (Config C st (m_lete x e1 e2) :: l) FUEL);
-      destruct (eval C st e1 [Config C st (m_lete x e1 e2)] FUEL);
-      try (rewrite HINT1 in H); try rewrite HINT1';
-      try (simpl in *; destruct H as [?|[[?|?]|?]]; eauto; inversion H; fail);
-      try (inversion contra; fail).
-      destruct contra as [RR [RR' CONTAINED]]. rewrite RR in *. rewrite RR' in *. clear RR RR'.
-      destruct v;
-      try (rewrite HINT1 in H; rewrite HINT1'; destruct H as [?|[[?|?]|?]]; simpl in *; eauto; inversion H). destruct st0.
-      specialize (IHFUEL (C [|dy_binde x t ([||])|])
-                         (ST (t !-> ev; mem) (tick C (ST mem t) x ev))
-                         e2 reached cf) as HINT2'.
-      specialize (IHFUEL (C [|dy_binde x t ([||])|])
-                         (ST (t !-> ev; mem) (tick C (ST mem t) x ev))
-                         e2 reached0 cf) as HINT2.
-      pose proof (reach_same FUEL (C [|dy_binde x t ([||])|])
-                                  (ST (t !-> ev; mem) (tick C (ST mem t) x ev))
-                                  e2 reached0 reached CONTAINED) as contra.
-      clear CONTAINED.
-      destruct (eval (C [|dy_binde x t ([||])|])
-                     (ST (t !-> ev; mem) (tick C (ST mem t) x ev))
-                     e2 reached FUEL);
-      destruct (eval (C [|dy_binde x t ([||])|])
-                     (ST (t !-> ev; mem) (tick C (ST mem t) x ev))
-                     e2 reached0 FUEL);
-      try (rewrite HINT2 in H); try rewrite HINT2';
-      try (rewrite HINT1 in H); try rewrite HINT1';
-      try (simpl in *; destruct H as [?|[[[?|?]|?]|?]]; eauto; inversion H; fail);
-      try (inversion contra; fail).
-      destruct contra as [RR [RR' CONTAINED]]. rewrite RR in *. rewrite RR' in *. clear RR RR'.
-      destruct v; rewrite HINT2 in H; try rewrite HINT2';
-      rewrite HINT1 in H; try rewrite HINT1';
-      simpl in *; destruct H as [?|[[[?|?]|?]|?]]; eauto; inversion H.
-    + specialize (IHFUEL C st e1 (Config C st (m_letm M e1 e2) :: l) cf) as HINT1'.
-      specialize (IHFUEL C st e1 [Config C st (m_letm M e1 e2)] cf) as HINT1.
-      assert (forall cf, In cf [Config C st (m_letm M e1 e2)] ->
-                         In cf (Config C st (m_letm M e1 e2) :: l)) as CONTAINED.
-      { intros; simpl in *; destruct H0; eauto. inversion H0. }
-      pose proof (reach_same FUEL C st e1 [Config C st (m_letm M e1 e2)] (Config C st (m_letm M e1 e2) :: l) CONTAINED) as contra.
-      clear CONTAINED.
-      destruct (eval C st e1 (Config C st (m_letm M e1 e2) :: l) FUEL);
-      destruct (eval C st e1 [Config C st (m_letm M e1 e2)] FUEL);
-      try (rewrite HINT1 in H); try rewrite HINT1';
-      try (simpl in *; destruct H as [?|[[?|?]|?]]; eauto; inversion H; fail);
-      try (inversion contra; fail).
-      destruct contra as [RR [RR' CONTAINED]]. rewrite RR in *. rewrite RR' in *. clear RR RR'.
-      destruct v;
-      try (rewrite HINT1 in H; rewrite HINT1'; destruct H as [?|[[?|?]|?]]; simpl in *; eauto; inversion H).
-      specialize (IHFUEL (C [|dy_bindm M mv ([||])|]) st0 e2 reached cf) as HINT2'.
-      specialize (IHFUEL (C [|dy_bindm M mv ([||])|]) st0 e2 reached0 cf) as HINT2.
-      pose proof (reach_same FUEL (C [|dy_bindm M mv ([||])|]) st0 e2 reached0 reached CONTAINED) as contra.
-      clear CONTAINED.
-      destruct (eval (C [|dy_bindm M mv ([||])|]) st0 e2 reached FUEL);
-      destruct (eval (C [|dy_bindm M mv ([||])|]) st0 e2 reached0 FUEL);
-      try (rewrite HINT2 in H); try rewrite HINT2';
-      try (rewrite HINT1 in H); try rewrite HINT1';
-      try (simpl in *; destruct H as [?|[[[?|?]|?]|?]]; eauto; inversion H; fail);
-      try (inversion contra; fail).
-      destruct contra as [RR [RR' CONTAINED]]. rewrite RR in *. rewrite RR' in *. clear RR RR'.
-      destruct v; rewrite HINT2 in H; rewrite HINT2';
-      rewrite HINT1 in H; rewrite HINT1';
-      simpl in *; destruct H as [?|[[[?|?]|?]|?]]; eauto; inversion H.
+  rename H into ET. rename H0 into OT. rename H1 into TT.
+  induction FUEL; intros;
+  assert (forall cf, In cf [Cf e C m t] ->
+            In cf (Cf e C m t :: l)) as CONTAINED;
+  try (intros; simpl in *; destruct H; eauto; contradict);
+  simpl; split; intros SPLIT.
+  { destruct SPLIT; eauto. }
+  { destruct SPLIT as [?|[?|?]]; eauto. contradict. }
+  - destruct e;
+    try (
+      (* trivial cases *)
+      lazymatch goal with 
+      | |- context [eval _ _ _ _ _ _] => fail
+      | _ => idtac
+      end;
+      repeat des_hyp; simpl in *;
+      try destruct SPLIT as [?|[?|?]];
+      try destruct SPLIT as [?|?]; eauto);
+    separate_reach_tac cf IHFUEL HINT1 HINT1' CONTAINED RR;
+    des_goal; des_hyp;
+    try (destruct RR as [? [? [? RR]]]; subst; des_hyp);
+    try (rewrite HINT1 in SPLIT;
+      destruct SPLIT as [[?|?]|?]; eauto;
+      right; rewrite HINT1'; simpl; eauto);
+    separate_reach_tac cf IHFUEL HINT2 HINT2' RR RR';
+    des_hyp; try des_goal; des_hyp;
+    try (destruct RR' as [? [? [? RR']]]; subst; try des_hyp);
+    try (rewrite HINT2 in SPLIT; destruct SPLIT as [SPLIT|?];
+      try (rewrite HINT1 in SPLIT; destruct SPLIT as [[?|?]|?]);
+      eauto;
+      rewrite HINT2'; rewrite HINT1'; simpl; eauto).
+    separate_reach_tac cf IHFUEL HINT3 HINT3' RR' RR''.
+    des_goal; des_hyp;
+    try (destruct RR'' as [? [? [? RR'']]]; subst; des_hyp);
+    try (rewrite HINT3 in SPLIT; destruct SPLIT as [SPLIT|?];
+      try (rewrite HINT2 in SPLIT; destruct SPLIT as [SPLIT|?];
+        try (rewrite HINT1 in SPLIT; destruct SPLIT as [[?|?]|?]));
+      eauto;
+      rewrite HINT3'; rewrite HINT2'; rewrite HINT1'; simpl; eauto 7).
+  - destruct e;
+    try (
+      (* trivial cases *)
+      lazymatch goal with 
+      | |- context [eval _ _ _ _ _ _] => fail
+      | _ => idtac
+      end;
+      repeat des_hyp; simpl in *;
+      try destruct SPLIT as [?|[?|[?|?]]];
+      try destruct SPLIT as [?|[?|?]];
+      try destruct SPLIT as [?|?]; eauto; contradict);
+    separate_reach_tac cf IHFUEL HINT1 HINT1' CONTAINED RR;
+    des_hyp; des_goal; try contradict;
+    try (destruct RR as [? [? [? RR]]]; subst; des_hyp);
+    try rewrite HINT1 in SPLIT; 
+    try destruct SPLIT as [?|[[?|?]|?]];
+    try rewrite HINT1';
+    simpl in *; eauto; try contradict;
+    try destruct ev;
+    separate_reach_tac cf IHFUEL HINT2 HINT2' RR RR';
+    des_hyp; des_goal; try contradict;
+    try (destruct RR' as [? [? [? RR']]]; subst; des_hyp);
+    try rewrite HINT2 in SPLIT;
+    try destruct SPLIT as [?|[SPLIT|?]];
+    try rewrite HINT1 in SPLIT;
+    try destruct SPLIT as [[?|?]|?];
+    try rewrite HINT2'; try rewrite HINT1';
+    simpl in *; eauto; try contradict.
+    separate_reach_tac cf IHFUEL HINT3 HINT3' RR' RR'';
+    des_hyp; repeat des_goal; try contradict;
+    try (destruct RR'' as [? [? [? RR'']]]; subst);
+    try rewrite HINT3 in SPLIT;
+    try destruct SPLIT as [?|[SPLIT|?]];
+    try rewrite HINT2 in SPLIT;
+    try destruct SPLIT as [SPLIT|?];
+    try rewrite HINT1 in SPLIT;
+    try destruct SPLIT as [[?|?]|?];
+    try rewrite HINT3'; try rewrite HINT2'; try rewrite HINT1';
+    simpl in *; eauto 7; try contradict.
 Qed.
 
+(*
 Lemma ReachR_well_defined_l :
   forall `{TIME : time T} (C : @dy_ctx T) st e C' st' e' (R : <| C st e ~> C' st' e' |>),
     exists FUEL,
@@ -1692,3 +1054,4 @@ Proof.
   intros; repeat split; inversion pf; inversion REACH; subst; eauto;
   try inversion H2.
 Qed.
+*)
