doc/coq/simple/Syntax.v
@@ -5,6 +5,7 @@ From Coq Require Export Arith.EqNat.
 From Coq Require Export Lia.
 From Coq Require Export Lists.List.
 From Coq Require Export Strings.String.
+From sflib Require Export sflib.
 
 Notation "x :: y" := (cons x y)
                      (at level 60, right associativity).
@@ -13,85 +14,175 @@ Notation "[ x ; .. ; y ]" := (cons x .. (cons y []) ..).
 Notation "x ++ y" := (app x y)
                      (at level 60, right associativity).
 
-Inductive expr_id :=
-  | eid (x : nat)
-.
+(* First, some basic definitions*)
+Ltac contradict :=
+  let contra := fresh "contra" in
+  assert False as contra; eauto 3; inversion contra.
 
-Inductive mod_id :=
-  | mid (M : nat)
-.
+Lemma __R__ : forall b, b = false <-> b <> true.
+Proof.
+  intros; split; intros; subst.
+  red; intros contra. inversion contra.
+  destruct b. contradict. eauto.
+Qed.
 
-Definition eq_eid id1 id2 :=
-  match id1, id2 with
-  | eid x1, eid x2 => x1 =? x2
+Ltac refl_bool :=
+  match goal with
+  | |- _ = false => rewrite __R__; unfold "<>"
+  | |- _ <> true => rewrite <- __R__
+  | _ => idtac
   end.
 
-Definition eq_mid id1 id2 :=
-  match id1, id2 with
-  | mid M1, mid M2 => M1 =? M2
+Ltac des_hyp :=
+  let DES := fresh "HDES" in
+  match goal with
+  | [H : context [?E || _] |- _] =>
+    destruct E eqn:DES; simpl in H;
+    try (inversion H; fail)
+  | [H : context [?E && _] |- _] =>
+    destruct E eqn:DES; simpl in H;
+    try (inversion H; fail)
+  | [H : context [match ?E with | _ => _ end] |- _] =>
+    destruct E eqn:DES; simpl in H;
+    try (inversion H; fail)
+  | _ => fail
   end.
 
-Lemma eq_eid_eq : forall x x',
-  eq_eid x x' = true <-> x = x'.
+Ltac des_goal :=
+  let DES := fresh "GDES" in
+  match goal with
+  | [|- context [?E || _]] =>
+    destruct E eqn:DES; simpl
+  | [|- context [?E && _]] =>
+    destruct E eqn:DES; simpl
+  | [|- context [match ?E with | _ => _ end]] =>
+    destruct E eqn:DES; simpl
+  | _ => fail
+  end.
+
+(* Types with decidable equality *)
+Class Eq T : Type :=
+{
+  eqb : T -> T -> bool;
+  eqb_eq : forall (t t' : T), eqb t t' = true <-> t = t';
+  eqb_neq : forall (t t' : T), eqb t t' = false <-> t <> t'
+}.
+
+Lemma eqb_neq_template T eqb 
+  (eqb_eq : forall (x x' : T), eqb x x' = true <-> x = x') : 
+  forall x x', eqb x x' = false <-> x <> x'.
 Proof.
-  intros. destruct x. destruct x'.
-  simpl. split; intros. 
-  rewrite Nat.eqb_eq in H.
-  rewrite H. eauto.
-  inversion H; subst. rewrite Nat.eqb_eq. eauto.
+  intros; split; intros contra.
+  - red; intros. rewrite <- eqb_eq in *. 
+    rewrite H in contra. inversion contra.
+  - destruct (eqb x x') eqn:EQ; try reflexivity.
+    exfalso. apply contra. rewrite <- eqb_eq. eauto.
 Qed.
 
-Lemma eq_eid_neq : forall x x',
-  eq_eid x x' = false <-> x <> x'.
+Lemma t_refl {T} `{Eq T} : forall t, eqb t t = true.
+Proof. intros; apply eqb_eq; eauto. Qed.
+
+Fixpoint Inb {T} `{Eq T} t (l : list T) :=
+  match l with
+  | [] => false
+  | hd :: tl => eqb hd t || Inb t tl
+  end.
+
+Lemma Inb_eq {T} `{Eq T} :
+  forall (l : list T) (t : T),
+    Inb t l = true <-> In t l.
 Proof.
-  intros. destruct x. destruct x'.
-  simpl. split; intros.
-  unfold not. intros.
-  rewrite Nat.eqb_neq in H. apply H. inversion H0. eauto.
-  rewrite Nat.eqb_neq. unfold not. intros. apply H. subst; eauto.
+  induction l; intros; simpl in *;
+  split; intros EQ; try contradict.
+  - repeat des_hyp;
+    simpl in *; try (inversion EQ; fail);
+    match goal with
+    | _ => left; rewrite <- eqb_eq; eauto; fail
+    | _ => right; rewrite <- IHl; eauto; fail
+    end.
+  - destruct EQ as [EQhd | EQtl].
+    subst. rewrite t_refl. eauto.
+    rewrite <- IHl in EQtl. rewrite EQtl.
+    destruct (eqb a t); eauto.
 Qed.
 
-Lemma eq_mid_eq : forall M M',
-  eq_mid M M' = true <-> M = M'.
+Lemma Inb_neq {T} `{Eq T} :
+  forall (l : list T) (t : T),
+    Inb t l = false <-> ~ (In t l).
 Proof.
-  intros. destruct M. destruct M'.
-  simpl. split; intros. 
-  rewrite Nat.eqb_eq in H.
-  rewrite H. eauto.
-  inversion H; subst. rewrite Nat.eqb_eq. eauto.
+  induction l; intros; simpl in *;
+  split; intros NEQ; eauto.
+  - red; intros EQ.
+    destruct (eqb a t) eqn:NEQhd;
+    destruct (Inb t l) eqn:NEQtl;
+    try (inversion NEQ; fail).
+    rewrite eqb_neq in NEQhd.
+    rewrite IHl in NEQtl.
+    destruct EQ as [EQhd | EQtl];
+    match goal with
+    | _ => apply NEQhd; eauto; fail
+    | _ => apply NEQtl; eauto; fail
+    end.
+  - destruct (eqb a t) eqn:NEQhd;
+    destruct (Inb t l) eqn:NEQtl; simpl;
+    match goal with
+    | _ => reflexivity; fail
+    | [H : eqb _ _ = true |- _] =>
+      rewrite eqb_eq in H
+    | [H : Inb _ _ = true |- _] =>
+      rewrite Inb_eq in H
+    end;
+    exfalso; apply NEQ; eauto.
 Qed.
 
-Lemma eq_mid_neq : forall M M',
-  eq_eid M M' = false <-> M <> M'.
-Proof.
-  intros. destruct M. destruct M'.
-  simpl. split; intros.
-  unfold not. intros.
-  rewrite Nat.eqb_neq in H. apply H. inversion H0. eauto.
-  rewrite Nat.eqb_neq. unfold not. intros. apply H. subst; eauto.
-Qed.
+(* Total order *)
+Class TotalOrder (T : Type) `{Eq T} : Type :=
+{
+  leb : T -> T -> bool;
+  leb_refl : forall t, leb t t = true;
+  leb_trans : forall t t' t'' (LE : leb t t' = true) (LE' : leb t' t'' = true), leb t t'' = true;
+  leb_sym : forall t t' (LE : leb t t' = true) (LE' : leb t' t = true), t = t';
+  leb_or : forall t t', leb t t' || leb t' t = true
+}.
+
+Definition lt {T} `{TotalOrder T} (t1 t2 : T) :=
+  leb t1 t2 = true /\ eqb t1 t2 = false.
+
+Notation "t1 '<' t2" := (lt t1 t2).
+
+(** Syntax of our language *)
+Definition ID := nat.
+
+Definition eqb_ID := Nat.eqb.
+
+Definition eqb_ID_eq := Nat.eqb_eq.
+
+Definition eqb_ID_neq := Nat.eqb_neq.
+
+Lemma ID_refl : forall x, eqb_ID x x = true.
+Proof. intros; apply eqb_ID_eq; eauto. Qed.
 
 Inductive tm :=
-  | e_var (x : expr_id)
-  | e_lam (x : expr_id) (e : tm)
+  | e_var (x : ID)
+  | e_lam (x : ID) (e : tm)
   | e_app (e1 : tm) (e2 : tm)
   | e_link (m : tm) (e : tm)
   | m_empty
-  | m_var (M : mod_id)
-  | m_lete (x : expr_id) (e : tm) (m : tm)
-  | m_letm (M : mod_id) (m1 : tm) (m2 : tm)
+  | m_var (M : ID)
+  | m_lete (x : ID) (e : tm) (m : tm)
+  | m_letm (M : ID) (m1 : tm) (m2 : tm)
 .
 
 Fixpoint eq_tm e e' :=
   match e, e' with
-  | e_var x, e_var x' => eq_eid x x'
-  | e_lam x e, e_lam x' e' => eq_eid x x' && eq_tm e e'
+  | e_var x, e_var x' => eqb_ID x x'
+  | e_lam x e, e_lam x' e' => eqb_ID x x' && eq_tm e e'
   | e_app e1 e2, e_app e1' e2' => eq_tm e1 e1' && eq_tm e2 e2'
   | e_link m e, e_link m' e' => eq_tm m m' && eq_tm e e'
   | m_empty, m_empty => true
-  | m_var M, m_var M' => eq_mid M M'
-  | m_lete x e m, m_lete x' e' m' => eq_eid x x' && eq_tm e e' && eq_tm m m'
-  | m_letm M m1 m2, m_letm M' m1' m2' => eq_mid M M' && eq_tm m1 m1' && eq_tm m2 m2'
+  | m_var M, m_var M' => eqb_ID M M'
+  | m_lete x e m, m_lete x' e' m' => eqb_ID x x' && eq_tm e e' && eq_tm m m'
+  | m_letm M m1 m2, m_letm M' m1' m2' => eqb_ID M M' && eq_tm m1 m1' && eq_tm m2 m2'
   | _, _ => false
   end.
 
@@ -99,74 +190,66 @@ Lemma eq_tm_eq : forall e e', eq_tm e e' = true <-> e = e'.
 Proof.
   induction e; intros; split; intros EQ; simpl in *;
   destruct e'; try (inversion EQ; fail);
-  try destruct (eq_eid x x0) eqn:EIDEQ;
-  try destruct (eq_mid M M0) eqn:MIDEQ;
-  try destruct (eq_tm e e') eqn:TMEQ;
-  try destruct (eq_tm e1 e'1) eqn:TMEQ1;
-  try destruct (eq_tm e2 e'2) eqn:TMEQ2;
-  inversion EQ;
-  try rewrite IHe in TMEQ;
-  try rewrite IHe1 in TMEQ1;
-  try rewrite IHe2 in TMEQ2;
-  try rewrite eq_eid_eq in *;
-  try rewrite eq_mid_eq in *;
-  subst; simpl;
-  try reflexivity;
-  try (rewrite <- EIDEQ; rewrite eq_eid_eq; reflexivity);
-  try (rewrite <- MIDEQ; rewrite eq_mid_eq; reflexivity);
-  try (rewrite <- TMEQ; rewrite IHe; reflexivity);
-  try (rewrite <- TMEQ1; rewrite IHe1; reflexivity);
-  try (rewrite <- TMEQ2; rewrite IHe2; reflexivity).
+  repeat des_hyp;
+  repeat match goal with
+  | [H : eqb_ID _ _ = true |- _] =>
+    rewrite eqb_ID_eq in H
+  | [H : eq_tm _ _ = true |- _] =>
+    repeat match goal with
+    | [RR : context [eq_tm _ _ = true <-> _] |- _] =>
+      rewrite RR in H
+    end
+  | _ => idtac
+  end; subst; try reflexivity;
+  inversion EQ; subst;
+  try rewrite ID_refl; simpl; try reflexivity;
+  repeat match goal with
+  | [H : context [eq_tm ?e _ = _] |- _] =>
+    match goal with
+    | [_ : eq_tm e e = true |- _] => fail
+    | _ =>
+      let RR := fresh "RR" in
+      assert (eq_tm e e = true) as RR;
+      try apply H; eauto; rewrite RR
+    end
+  | _ => fail
+  end.
 Qed.
 
-Inductive value : tm -> Prop :=
-  | v_fn x e : value (e_lam x e)
+(** Statics *)
+Inductive path :=
+  | pnil
+  | pe (x : ID) (tl : path)
+  | pm (M : ID) (tl : path)
+.
+
+Inductive value :=
+  | v_fn (x : ID) (e : tm)
+  | v_ptr (ptr : path -> bool)
 .
 
 Inductive st_ctx :=
   | st_hole
-  | st_binde (x : expr_id) (C : st_ctx)
-  | st_bindm (M : mod_id) (CM : st_ctx) (C : st_ctx)
+  | st_binde (x : ID) (C : st_ctx)
+  | st_bindm (M : ID) (CM : st_ctx) (C : st_ctx)
 .
 
-Fixpoint st_ctx_M (C : st_ctx) (M : mod_id) :=
+Notation "'[[|' '|]]'" := (st_hole) (at level 99).
+
+Fixpoint st_ctx_M (C : st_ctx) (M : ID) :=
   match C with
-  | st_hole => None
+  | [[||]] => None
   | st_binde _ C' => st_ctx_M C' M
   | st_bindm M' CM' C' =>
-    match st_ctx_M C' M with
-    | Some CM => Some CM
-    | None => if eq_mid M M' then Some CM' else None
-    end
+    if eqb_ID M M' then Some CM' else st_ctx_M C' M
   end.
-
-Fixpoint st_c_plugin (Cout : st_ctx) (Cin : st_ctx) :=
-  match Cout with
-  | st_hole => Cin
-  | st_binde x C' => st_binde x (st_c_plugin C' Cin)
-  | st_bindm M' CM' C' => st_bindm M' CM' (st_c_plugin C' Cin)
-  end.
-
-Lemma st_c_plugin_assoc : forall C1 C2 C3,
-  st_c_plugin (st_c_plugin C1 C2) C3 =
-  st_c_plugin C1 (st_c_plugin C2 C3). 
-Proof.
-  induction C1; eauto; 
-  intros; simpl; try rewrite IHC1; eauto.
-  rewrite IHC1_2. eauto.
-Qed.
-
-Notation "Cout '[[|' Cin '|]]'" := (st_c_plugin Cout Cin)
-                              (at level 100, Cin at next level, right associativity).
-
-Notation "'[[||]]'" := (st_hole) (at level 100).
 
 (* collect all static contexts reachable from the current configuration *)
 Fixpoint collect_ctx C e :=
   match e with
   | e_var x => (None, [C])
   | e_lam x e' => 
-    let ctx_body := snd (collect_ctx (C [[|st_binde x ([[||]])|]]) e') in
+    let ctx_body := snd (collect_ctx (st_binde x C) e') in
     (None, C :: ctx_body)
   | e_app e1 e2 =>
     let ctxs1 := snd (collect_ctx C e1) in
@@ -187,125 +270,65 @@ Fixpoint collect_ctx C e :=
     end
   | m_lete x e m' =>
     let ctxs_e := snd (collect_ctx C e) in
-    let (ctx_o, ctxs_m) := collect_ctx 
-                           (C [[|st_binde x ([[||]])|]]) m' in
+    let (ctx_o, ctxs_m) := collect_ctx (st_binde x C) m' in
     (ctx_o, ctxs_e ++ ctxs_m)
   | m_letm M m1 m2 =>
     match collect_ctx C m1 with
     | (Some C_M, ctxs_m1) => 
-      let (ctx_o, ctxs_m2) := collect_ctx
-                              (C [[|st_bindm M C_M ([[||]])|]]) m2 in
+      let (ctx_o, ctxs_m2) := collect_ctx (st_bindm M C_M C) m2 in
       (ctx_o, ctxs_m1 ++ ctxs_m2)
     | (None, ctxs_m1) => (None, ctxs_m1)
     end
   end.
 
-Lemma st_ctx_M_plugin :
-  forall Cout Cin M,
-    st_ctx_M (st_c_plugin Cout Cin) M =
-      match st_ctx_M Cin M with
-      | Some CM => Some CM
-      | None =>
-        match st_ctx_M Cout M with
-        | Some CM => Some CM
-        | None => None
-        end
-      end.
-Proof.
-  induction Cout; intros; simpl; eauto.
-  - destruct (st_ctx_M Cin M); eauto.
-  - specialize (IHCout2 Cin M0). 
-    destruct (st_ctx_M Cin M0). 
-    rewrite IHCout2. eauto. 
-    rewrite IHCout2.
-    destruct (st_ctx_M Cout2 M0). eauto.
-    assert (RR : forall Cout0 Cin0, 
-    st_ctx_M (st_c_plugin Cout0 Cin0) M0 = None -> st_ctx_M Cin0 M0 = None).
-    { induction Cout0; intros; simpl; eauto. 
-      simpl in H. apply IHCout0_2.
-      destruct (st_ctx_M (st_c_plugin Cout0_2 Cin0) M0).
-      inversion H. eauto. }
-    specialize (IHCout1 Cin M0).
-    rewrite (RR Cout2 Cin IHCout2) in IHCout1.
-    destruct (eq_mid M0 M).
-    eauto. eauto.
-Qed.
-
 Lemma collect_ctx_refl : forall e C, In C (snd (collect_ctx C e)).
 Proof.
-  induction e; intros; simpl; eauto.
-  - apply in_app_iff. left. eauto.
-  - remember (collect_ctx C e1) as ol. destruct ol as [o l].
-    specialize (IHe1 C). rewrite <- Heqol in IHe1.
-    destruct o; eauto. simpl in *.
-    destruct (collect_ctx C e2); simpl in *.
-    destruct (collect_ctx s e2); simpl in *. 
-    apply in_app_iff. left. eauto.
-  - destruct (st_ctx_M C M); simpl; left; eauto.
-  - destruct (collect_ctx (C [[|st_binde x ([[||]])|]]) e2).
-    apply in_app_iff. left. eauto.
-  - remember (collect_ctx C e1) as ol.
-    destruct ol as [o l]. specialize (IHe1 C). rewrite <- Heqol in IHe1.
-    destruct o; eauto.
-    destruct (collect_ctx (C [[|st_bindm M s ([[||]])|]]) e2).
-    apply in_app_iff. left. eauto.
+  induction e; intros; simpl; eauto;
+  repeat des_goal;
+  try apply in_app_iff; try left; eauto;
+  repeat match goal with
+  | [H : forall _ : st_ctx, In _ (snd (collect_ctx _ ?e)) |- _] =>
+    match goal with
+    | [RR : collect_ctx ?C e = _ |- _] =>
+      specialize (H C); rewrite RR in H
+    | _ => fail
+    end
+  | _ => fail
+  end; simpl in *; eauto.
 Qed.
 
-(* dynamic context *)
+(** Dynamics *)
 Inductive dy_ctx {time : Type} :=
   | dy_hole
-  | dy_binde (x: expr_id) (tx : time) (C : dy_ctx)
-  | dy_bindm (M : mod_id) (CM : dy_ctx) (C : dy_ctx)
+  | dy_binde (x : ID) (tx : time) (C : dy_ctx)
+  | dy_bindm (M : ID) (CM : dy_ctx) (C : dy_ctx)
 .
 
-Fixpoint dy_plugin_c {time : Type} (Cout : @dy_ctx time) (Cin : @dy_ctx time) :=
-  match Cout with
-  | dy_hole => Cin
-  | dy_binde x tx C' => dy_binde x tx (dy_plugin_c C' Cin)
-  | dy_bindm M CM C' => dy_bindm M CM (dy_plugin_c C' Cin)
-  end.
+Notation "'[|' '|]'" := (dy_hole) (at level 99).
 
-Fixpoint addr_x {time : Type} (C : @dy_ctx time) (x : expr_id) :=
+(* Auxiliary operators *)
+Fixpoint addr_x {time : Type} (C : @dy_ctx time) (x : ID) :=
   match C with
-  | dy_hole => None
+  | [||] => None
   | dy_binde x' tx' C' =>
-    match addr_x C' x with
-    | None => if eq_eid x x' then (Some tx') else None
-    | addr => addr
-    end
+    if eqb_ID x x' then (Some tx') else addr_x C' x
   | dy_bindm _ _ C' => addr_x C' x
   end.
 
-Fixpoint ctx_M {time : Type} (C : @dy_ctx time) (M : mod_id) :=
+Fixpoint ctx_M {time : Type} (C : @dy_ctx time) (M : ID) :=
   match C with
-  | dy_hole => None
+  | [||] => None
   | dy_binde _ _ C' => ctx_M C' M
   | dy_bindm M' CM' C' =>
-    match ctx_M C' M with
-    | Some CM => Some CM
-    | None => if eq_mid M M' then Some CM' else None
-    end
+    if eqb_ID M M' then Some CM' else ctx_M C' M
   end.
 
-(* a term, a context *)
-Inductive expr_value {time : Type} :=
-  | Closure (x : expr_id) (e : tm) (C : @dy_ctx time)
-.
-
-Inductive dy_value {time : Type} :=
-  | EVal (ev : @expr_value time)
-  | MVal (mv : @dy_ctx time)
-.
-
-Notation "Cout '[|' Cin '|]'" := (dy_plugin_c Cout Cin)
-                              (at level 100, Cin at next level, right associativity).
-Notation "'[||]'" := (dy_hole) (at level 100).
-
-Fixpoint In_ctx {T} (t : T) (C : @dy_ctx T) :=
+(* Auxiliary definition to aid proofs *)
+Fixpoint st_level (C : st_ctx) :=
   match C with
-  | [||] => False
-  | dy_binde _ t' C' => t = t' \/ In_ctx t C'
-  | dy_bindm _ C' C'' => In_ctx t C' \/ In_ctx t C''
+  | [[||]] => 0
+  | st_binde _ C' => S (st_level C')
+  | st_bindm _ C' C'' => S (Nat.max (st_level C') (st_level C''))
   end.
 
 Fixpoint dy_level {T} (C : @dy_ctx T) :=
@@ -315,616 +338,689 @@ Fixpoint dy_level {T} (C : @dy_ctx T) :=
   | dy_bindm _ C' C'' => S (Nat.max (dy_level C') (dy_level C''))
   end.
 
-Lemma c_plugin_assoc : forall {T} (C1 : @dy_ctx T) C2 C3, C1[| C2[| C3 |] |] = ((C1[|C2|])[|C3|]).
-Proof.
-  induction C1; eauto; 
-  intros; simpl; try rewrite IHC1; eauto.
-  rewrite IHC1_2. eauto.
-Qed.
-
 Fixpoint dy_to_st {T} (C : @dy_ctx T) :=
   match C with
-  | ([||]) => ([[||]])
+  | [||] => [[||]]
   | dy_binde x _ C' => st_binde x (dy_to_st C')
   | dy_bindm M CM C' => st_bindm M (dy_to_st CM) (dy_to_st C')
   end.
 
-Lemma in_plugin_iff :
-  forall {T} (t : T) (Cout Cin : @dy_ctx T),
-    In_ctx t (Cout[|Cin|]) <-> (In_ctx t Cout \/ In_ctx t Cin).
+Lemma st_dy_level_eq {T} :
+  forall (C : @dy_ctx T), dy_level C = st_level (dy_to_st C).
 Proof.
-  intros. revert Cin.
-  induction Cout; intros; split; simpl; intros H; 
-  try rewrite IHCout in H;
-  try rewrite IHCout2 in H;
-  try rewrite IHCout;
-  try rewrite IHCout2;
-  try destruct H as [? | [? | ?]];
-  try destruct H as [[? | ?] | ?];
-  eauto.
-  destruct H; try assumption; inversion H. 
+  induction C; simpl; eauto.
 Qed.
 
-Lemma dy_to_st_plugin :
-  forall {T} (Cout : @dy_ctx T) Cin,
-    dy_to_st (Cout[|Cin|]) = st_c_plugin (dy_to_st Cout) (dy_to_st Cin).
-Proof.
-  induction Cout; intros; simpl; try rewrite IHCout; eauto.
-  rewrite IHCout2. eauto.
-Qed. 
-
-Lemma mod_is_static_none : forall {T} (dC : @dy_ctx T) (M : mod_id),
+Lemma mod_is_static_none : forall {T} (dC : @dy_ctx T) (M : ID),
   (ctx_M dC M = None <-> st_ctx_M (dy_to_st dC) M = None).
 Proof. 
-  intros. repeat split. 
-  - induction dC; simpl; eauto.
-    destruct (ctx_M dC2 M). intros H; inversion H.
-    specialize (IHdC2 eq_refl). rewrite IHdC2.
-    destruct (eq_mid M M0). intros H; inversion H. eauto.
-  - induction dC; simpl; eauto.
-    destruct (st_ctx_M (dy_to_st dC2) M). intros H; inversion H.
-    specialize (IHdC2 eq_refl). rewrite IHdC2.
-    destruct (eq_mid M M0). intros H; inversion H. eauto.
+  intros. repeat split; induction dC; simpl; eauto;
+  repeat des_goal; eauto;
+  match goal with
+  | _ => let H := fresh "H" in intro H; inversion H
+  | _ => idtac
+  end.
 Qed.
 
-Lemma mod_is_static_some : forall {T} (dC : @dy_ctx T) (M : mod_id),
+Lemma mod_is_static_some : forall {T} (dC : @dy_ctx T) (M : ID),
   (forall v, ctx_M dC M = Some v -> st_ctx_M (dy_to_st dC) M = Some (dy_to_st v)) /\
   (forall v, st_ctx_M (dy_to_st dC) M = Some v -> exists dv, dy_to_st dv = v /\ ctx_M dC M = Some dv).
 Proof.
-  intros; split. 
-  - induction dC; simpl; intros; eauto.
-    + inversion H.
-    + remember (ctx_M dC2 M) as v2. destruct v2.
-      specialize (IHdC2 v H). rewrite IHdC2. eauto.
-      symmetry in Heqv2. rewrite mod_is_static_none in Heqv2.
-      rewrite Heqv2. destruct (eq_mid M M0); inversion H; eauto.
-  - induction dC; simpl; intros; eauto.
-    + inversion H.
-    + remember (st_ctx_M (dy_to_st dC2) M) as v2. destruct v2.
-      specialize (IHdC2 v H). inversion IHdC2. exists x.
-      destruct H0. split. assumption. rewrite H1. eauto.
-      remember (ctx_M dC2 M) as v2. destruct v2;
-      symmetry in Heqv2; rewrite <- mod_is_static_none in Heqv2.
-      rewrite Heqv2 in Heqv0. inversion Heqv0.
-      destruct (eq_mid M M0). inversion H.
-      exists dC1. eauto. inversion H.
+  intros; split; induction dC; simpl; intros; eauto;
+  match goal with
+  | [H : None = Some _ |- _] => inversion H
+  | [H : Some _ = None |- _] => inversion H
+  | _ => repeat des_goal; eauto;
+    match goal with
+    | [H : Some _ = Some _ |- _] =>
+      inversion H; subst; eauto
+    | _ => idtac
+    end
+  end.
 Qed.
 
-Fixpoint trans_ctx {CT AT} (α : CT -> AT) (C : @dy_ctx CT) :=
-  match C with
-  | [||] => [||]
-  | dy_binde x t C' => dy_binde x (α t) (trans_ctx α C')
-  | dy_bindm M CM C' => dy_bindm M (trans_ctx α CM) (trans_ctx α C')
-  end.
-
-Definition trans_v {CT AT} (α : CT -> AT) (v : @expr_value CT) :=
-  match v with
-  | Closure x e C => Closure x e (trans_ctx α C)
-  end.
-
-Definition trans_V {CT AT} (α : CT -> AT) (V : @dy_value CT) :=
-  match V with
-  | EVal v => EVal (trans_v α v)
-  | MVal C => MVal (trans_ctx α C)
-  end.
-
-Definition trans_mem {CT AT} (α : CT -> AT) (mem : CT -> option (@expr_value CT)) (abs_mem : AT -> list (@expr_value AT)) :=
-  forall abs_t abs_v,
-    (In abs_v (abs_mem abs_t) <->
-      exists t v, trans_v α v = abs_v /\ α t = abs_t /\ mem t = Some v)
+(* More semantic domains *)
+Inductive expr_value {time : Type} :=
+  | Closure (x : ID) (e : tm) (C : @dy_ctx time)
 .
 
-Lemma trans_ctx_addr :
+Inductive dy_value {time : Type} :=
+  | EVal (ev : @expr_value time)
+  | MVal (mv : @dy_ctx time)
+.
+
+Definition memory {T} := T -> option (@expr_value T).
+
+Definition amemory {T} := T -> list (@expr_value T).
+
+Inductive config {T} :=
+  | Cf (e : tm) (C : @dy_ctx T) (m : @memory T) (t : T)
+  | Rs (V : @dy_value T) (m : @memory T) (t : T)
+.
+
+Inductive aconfig {T} :=
+  | ACf (e : tm) (abs_C : @dy_ctx T) (abs_m : @amemory T) (abs_t : T)
+  | ARs (abs_V : @dy_value T) (abs_m : @amemory T) (abs_t : T)
+.
+
+(* Definitions for the (finite) supports *)
+Fixpoint supp_C {T} (C : @dy_ctx T) (t : T) :=
+  match C with
+  | [||] => False
+  | dy_binde _ t' C' => t = t' \/ supp_C C' t
+  | dy_bindm _ C' C'' => supp_C C' t \/ supp_C C'' t
+  end.
+
+Definition supp_v {T} (v : @expr_value T) :=
+  match v with
+  | Closure _ _ C => supp_C C
+  end.
+
+Definition supp_V {T} (V : @dy_value T) :=
+  match V with
+  | EVal ev => supp_v ev
+  | MVal mv => supp_C mv
+  end.
+
+Definition supp_m {T} (m : memory) (t : T) :=
+  exists addr v, m addr = Some v /\ (addr = t \/ supp_v v t).
+
+Definition supp_ρ {T} (ρ : config) (t : T) :=
+  match ρ with
+  | Cf _ C m time => supp_C C t \/ supp_m m t \/ time = t
+  | Rs V m time => supp_V V t \/ supp_m m t \/ time = t
+  end.
+
+(** Observational equivalence *)
+Inductive view {T} :=
+  | Ctx (C : @dy_ctx T)
+  | Ptr (t : T) (* for imperative extensions *)
+  | Opq (* cannot observe more *)
+.
+
+Fixpoint obs_view {T : Type}
+  (V : @dy_value T) (m : @memory T) (p : path) :=
+  match p with
+  | pnil =>
+    match V with
+    | EVal (Closure x e C) => Ctx C
+    | MVal C => Ctx C
+    end
+  | pe x tl =>
+    match obs_view V m tl with
+    | Ctx C =>
+      match addr_x C x with
+      | None => Opq
+      | Some t =>
+        match m t with
+        | None => Opq
+        | Some (Closure x e C) => Ctx C
+        end
+      end
+    | _ => Opq
+    end
+  | pm M tl =>
+    match obs_view V m tl with
+    | Ctx C =>
+      match ctx_M C M with
+      | None => Opq
+      | Some C => Ctx C
+      end
+    | _ => Opq
+    end
+  end.
+
+Definition ptr_of_t {T} `{Eq T}
+  (V : @dy_value T) (m : @memory T) (t : T) (p : path) :=
+  match obs_view V m p with
+  | Ptr t' => eqb t t'
+  | _ => false
+  end.
+
+Fixpoint observe {T} `{Eq T}
+  (V : @dy_value T) (m : @memory T) (p : path) :=
+  match p with
+  | pnil =>
+    match V with
+    | EVal (Closure x e C) =>
+      (Ctx C, [v_fn x e])
+    | MVal C => (Ctx C, [])
+    end
+  | pe x tl =>
+    match observe V m tl with
+    | (Ctx C, obs) =>
+      match addr_x C x with
+      | None => (Opq, obs)
+      | Some t =>
+        match m t with
+        | None => (Opq, obs)
+        | Some (Closure x e C) =>
+          (Ctx C, (v_fn x e) :: obs)
+        end
+      end
+    | (_, obs) => (Opq, obs)
+    end
+  | pm M tl =>
+    match observe V m tl with
+    | (Ctx C, obs) =>
+      match ctx_M C M with
+      | None => (Opq, obs)
+      | Some C => (Ctx C, obs)
+      end
+    | (_, obs) => (Opq, obs)
+    end
+  end.
+
+Lemma eq_obs_view {T} `{Eq T} :
+  forall V m p, fst (observe V m p) = obs_view V m p.
+Proof.
+  intros.
+  induction p; simpl;
+  repeat des_goal; simpl in *; clarify; eauto.
+Qed.
+
+Definition Observe {T} `{Eq T} 
+  (V : @dy_value T) (m : @memory T) (p : path) :=
+  snd (observe V m p).
+
+Definition equiv {T T'} `{Eq T} `{Eq T'}
+  (V : @dy_value T) (m : @memory T) (V' : @dy_value T') (m' : @memory T') :=
+  forall p, Observe V m p = Observe V' m' p.
+
+Notation "'<|' V1 m1 '≃' V2 m2 '|>'" :=
+  (equiv V1 m1 V2 m2)
+  (at level 10, V1 at next level, m1 at next level, V2 at next level, m2 at next level).
+
+Fixpoint aobs_view {T : Type}
+  (V : @dy_value T) (m : @amemory T) (p : path) :=
+  match p with
+  | pnil =>
+    match V with
+    | EVal (Closure x e C) => [Ctx C]
+    | MVal C => [Ctx C]
+    end
+  | pe x tl =>
+    List.fold_left (fun acc single_view =>
+    let new_views := match single_view with
+    | Ctx C =>
+      match addr_x C x with
+      | None => [Opq]
+      | Some t =>
+        List.fold_left (fun acc v => 
+        let new_view := match v with
+        | Closure x e C => Ctx C
+        end in
+        new_view :: acc) (m t) [Opq]
+      end
+    | _ => [Opq]
+    end in
+    new_views ++ acc) (aobs_view V m tl) []
+  | pm M tl =>
+    List.fold_left (fun acc single_view =>
+    let new_view := match single_view with
+    | Ctx C =>
+      match ctx_M C M with
+      | None => Opq
+      | Some C => Ctx C
+      end
+    | _ => Opq
+    end in
+    new_view :: acc) (aobs_view V m tl) []
+  end.
+
+Definition aptr_of_t {T} `{Eq T}
+  (V : @dy_value T) (m : @amemory T) (t : T) (p : path) :=
+  Inb t (List.fold_left (fun acc single_view =>
+    match single_view with
+    | Ptr t => t :: acc
+    | _ => acc
+    end) (aobs_view V m p) []).
+
+Fixpoint aobserve {T : Type} 
+  (V : @dy_value T) (m : @amemory T) (p : path) :=
+  match p with
+  | pnil =>
+    match V with
+    | EVal (Closure x e C) =>
+      [(Ctx C, [v_fn x e])]
+    | MVal C => [(Ctx C, [])]
+    end
+  | pe x tl =>
+    List.fold_left (fun acc single_trace =>
+    let new_traces := match single_trace with
+    | (Ctx C, obs) =>
+      match addr_x C x with
+      | None => [(Opq, obs)]
+      | Some t =>
+        List.fold_left (fun acc v =>
+          let new_trace := match v with
+          | Closure x e C =>
+            (Ctx C, (v_fn x e) :: obs)
+          end in
+          new_trace :: acc) (m t) [(Opq, obs)]
+      end
+    | (_, obs) => [(Opq, obs)]
+    end in
+    new_traces ++ acc) (aobserve V m tl) []
+  | pm M tl =>
+    List.fold_left (fun acc single_trace =>
+    let new_trace := match single_trace with
+    | (Ctx C, obs) =>
+      match ctx_M C M with
+      | None => (Opq, obs)
+      | Some C => (Ctx C, obs)
+      end
+    | (_, obs) => (Opq, obs)
+    end in
+    new_trace :: acc) (aobserve V m tl) []
+  end.
+
+Lemma union_map_comm A B :
+  forall (l acc : list A) (f : A -> B) g g'
+    (RR : forall a x, map f (g a x) = g' (map f a) (f x)),
+  map f (fold_left g l acc) = fold_left g' (map f l) (map f acc).
+Proof.
+  induction l; intros; simpl; eauto.
+  rewrite <- RR.
+  apply IHl. eauto.
+Qed.
+
+Lemma fold_map_comm T A B :
+  forall (l : list T) (acc : list A) (f : A -> B) g g'
+    (RR : forall a x, map f (g a x) = g' (map f a) x),
+  map f (fold_left g l acc) = fold_left g' l (map f acc).
+Proof.
+  induction l; intros; simpl; eauto.
+  rewrite <- RR.
+  apply IHl. eauto.
+Qed.
+
+Lemma app_map_comm A B :
+  forall (l1 l2 : list A) (f : A -> B),
+    map f (l1 ++ l2) = map f l1 ++ map f l2.
+Proof.
+  induction l1; simpl; eauto.
+  intros. rewrite IHl1. eauto.
+Qed.
+
+Lemma cut_tail_app T :
+  forall (tl l l' : list T),
+    l ++ tl = l' ++ tl <-> l = l'.
+Proof.
+  assert (forall (ll : list T), ll ++ [] = ll) as RR.
+  { induction ll; simpl; eauto. rewrite IHll. eauto. }
+  assert (forall (ll ll' : list T) (t : T) (EQ : ll ++ [t] = ll' ++ [t]), ll = ll').
+  { 
+    induction ll; induction ll'; intros; simpl in *; eauto;
+    inversion EQ; subst;
+    match goal with
+    | [H : [] = _ ++ [?t] |- _] =>
+      assert (In t []) as contra;
+      try (rewrite H; rewrite in_app_iff; right; simpl; eauto);
+      inversion contra
+    | [H : _ ++ [?t] = [] |- _] =>
+      assert (In t []) as contra;
+      try (rewrite <- H; rewrite in_app_iff; right; simpl; eauto);
+      inversion contra
+    | [H : _ ++ [?t] = _ ++ [?t] |- _] =>
+      apply IHll in H; subst; eauto
+    end. 
+  }
+  induction tl.
+  - intros. rewrite RR. rewrite RR. eauto.
+  - intros.
+    replace (a :: tl) with ([a] ++ tl) by reflexivity.
+    rewrite app_assoc. rewrite app_assoc.
+    rewrite IHtl.
+    split; eauto.
+    intros; subst; eauto.
+Qed.
+
+Lemma eq_aobs_view {T} `{Eq T} :
+  forall V m p, List.map fst (aobserve V m p) = @aobs_view T V m p.
+Proof.
+  intros.
+  induction p; simpl;
+  repeat des_goal; simpl in *; clarify; eauto;
+  rewrite <- IHp; apply union_map_comm;
+  induction a; intros; simpl; repeat des_goal; eauto;
+  rewrite app_map_comm;
+  rewrite cut_tail_app;
+  replace [Opq] with (map fst [(@Opq T, l)]) by reflexivity;
+  apply fold_map_comm; intros;
+  match goal with
+  | [l : list _ |- _] => 
+    (* most recently introduced *) induction l
+  end; repeat des_goal; simpl; eauto.
+Qed.
+
+Definition AObserve {T : Type} 
+  (V : @dy_value T) (m : @amemory T) (p : path) :=
+  List.map snd (aobserve V m p).
+
+Definition aequiv {T T'}
+  (V : @dy_value T) (m : @amemory T) (V' : @dy_value T') (m' : @amemory T') :=
+  forall (p : path) (vl : list value),
+    In vl (AObserve V m p) <-> In vl (AObserve V' m' p).
+
+Notation "'<|' V1 m1 '≃#' V2 m2 '|>'" :=
+  (aequiv V1 m1 V2 m2)
+  (at level 10, V1 at next level, m1 at next level, V2 at next level, m2 at next level).
+
+(* Translation of timestamps *)
+Fixpoint trans_C {T T'} (α : T -> T') (C : @dy_ctx T) :=
+  match C with
+  | [||] => [||]
+  | dy_binde x t C' => dy_binde x (α t) (trans_C α C')
+  | dy_bindm M CM C' => dy_bindm M (trans_C α CM) (trans_C α C')
+  end.
+
+Definition trans_v {T T'} (α : T -> T') (v : @expr_value T) :=
+  match v with
+  | Closure x e C => Closure x e (trans_C α C)
+  end.
+
+Definition trans_V {T T'} (α : T -> T') (V : @dy_value T) :=
+  match V with
+  | EVal v => EVal (trans_v α v)
+  | MVal C => MVal (trans_C α C)
+  end.
+
+Definition trans_m {T T'} (α : T -> T') (m : @memory T) (m' : @memory T') :=
+  forall t' v',
+    (m' t' = Some v' <->
+      exists t v, trans_v α v = v' /\ α t = t' /\ m t = Some v)
+.
+
+Definition abstract_m {CT AT} (α : CT -> AT) (m : @memory CT) (am : @amemory AT) :=
+  forall abs_t abs_v,
+    (In abs_v (am abs_t) <->
+      exists t v, trans_v α v = abs_v /\ α t = abs_t /\ m t = Some v)
+.
+
+Definition trans_am {AT AT'} (α : AT -> AT') (am : @amemory AT) (am' : @amemory AT') :=
+  forall abs_t' abs_v',
+    (In abs_v' (am' abs_t') <->
+      exists abs_t abs_v, trans_v α abs_v = abs_v' /\ α abs_t = abs_t' /\ In abs_v (am abs_t))
+.
+
+Definition trans_ρ {T T'} (α : T -> T') (ρ : @config T) (ρ' : @config T') :=
+  match ρ, ρ' with
+  | Cf e C m t, Cf e' C' m' t' =>
+    e = e' /\ trans_C α C = C' /\ trans_m α m m' /\ α t = t'
+  | Rs V m t, Rs V' m' t' =>
+    trans_V α V = V' /\ trans_m α m m' /\ α t = t'
+  | _, _ => False
+  end.
+
+Definition abstract_ρ {CT AT} (α : CT -> AT) (ρ : @config CT) (aρ : @aconfig AT) :=
+  match ρ, aρ with
+  | Cf e C m t, ACf e' C' m' t' =>
+    e = e' /\ trans_C α C = C' /\ abstract_m α m m' /\ α t = t'
+  | Rs V m t, ARs V' m' t' =>
+    trans_V α V = V' /\ abstract_m α m m' /\ α t = t'
+  | _, _ => False
+  end.
+
+Definition trans_aρ {T T'} (α : T -> T') (aρ : @aconfig T) (aρ' : @aconfig T') :=
+  match aρ, aρ' with
+  | ACf e C m t, ACf e' C' m' t' =>
+    e = e' /\ trans_C α C = C' /\ trans_am α m m' /\ α t = t'
+  | ARs V m t, ARs V' m' t' =>
+    trans_V α V = V' /\ trans_am α m m' /\ α t = t'
+  | _, _ => False
+  end.
+
+(* Lemmas on translation *)
+Lemma trans_C_addr :
   forall {CT AT} (α : CT -> AT) C x,
-    addr_x (trans_ctx α C) x = 
+    addr_x (trans_C α C) x = 
       match (addr_x C x) with 
       | None => None 
       | Some addr => Some (α addr) 
       end.
 Proof.
   induction C; eauto.
-  - intros. specialize (IHC x0).
-    simpl. rewrite IHC.
-    destruct (addr_x C x0); simpl; eauto.
-    destruct (eq_eid x0 x); eauto.
+  intros. simpl.
+  destruct (eqb_ID x0 x); eauto.
 Qed.
 
-Lemma trans_ctx_ctx_M :
+Lemma trans_C_ctx_M :
   forall {CT AT} C (α : CT -> AT) abs_C M C_M
         (ACCESS : ctx_M C M = Some C_M)
-        (TRANS : trans_ctx α C = abs_C),
-    ctx_M abs_C M = Some (trans_ctx α C_M).
+        (TRANS : trans_C α C = abs_C),
+    ctx_M abs_C M = Some (trans_C α C_M).
 Proof.
-  assert (forall {CT AT} C (α : CT -> AT) M,
-    match ctx_M (trans_ctx α C) M with
-    | Some _ => 
-      match ctx_M C M with
-      | Some _ => True
-      | None => False
-      end
-    | None =>
-      match ctx_M C M with
-      | Some _ => False
-      | None => True
-      end
-    end) as A.
-  {
-    induction C; intros; simpl; eauto; try apply IHC.
-    destruct (eq_mid M0 M); 
-    remember (ctx_M (trans_ctx α C2) M0) as ctx';
-    destruct ctx';
-    specialize (IHC2 α M0);
-    rewrite <- Heqctx' in IHC2;
-    destruct (ctx_M C2 M0);
-    try inversion IHC2; eauto.
-  }
-  intros. revert C α abs_C M C_M ACCESS TRANS. 
-  induction C; intros; simpl in *; eauto.
+  induction C; intros; simpl in *.
   - inversion ACCESS.
   - rewrite <- TRANS. simpl. apply IHC; eauto.
   - rewrite <- TRANS. simpl.
-    remember (ctx_M (trans_ctx α C2) M0) as ctx1.
-    destruct ctx1; try (inversion ACCESS; fail).
-    + specialize (A CT AT C2 α M0).
-      rewrite <- Heqctx1 in A.
-      remember (ctx_M C2 M0) as ctx2; destruct ctx2;
-      inversion A; inversion ACCESS; subst.
-      rewrite Heqctx1. apply IHC2; eauto.
-    + specialize (A CT AT C2 α M0).
-      rewrite <- Heqctx1 in A.
-      remember (ctx_M C2 M0) as ctx2; destruct ctx2;
-      inversion A; destruct (eq_mid M0 M);
-      inversion ACCESS; subst; eauto.
+    destruct (eqb_ID M0 M); eauto.
+    inversion ACCESS; eauto.
 Qed.
 
-Lemma plugin_trans_ctx :
-  forall {CT AT} Cout Cin (α : CT -> AT),
-    trans_ctx α (Cout[|Cin|]) = (trans_ctx α Cout [|trans_ctx α Cin|]).
-Proof.
-  induction Cout; intros; simpl; 
-  try rewrite IHCout; try rewrite IHCout1; try rewrite IHCout2;
-  eauto.
-Qed.
-
-Class Eq T : Type :=
-{
-  eqb : T -> T -> bool;
-  eqb_eq : forall (t t' : T), eqb t t' = true <-> t = t';
-  eqb_neq : forall (t t' : T), eqb t t' = false <-> t <> t'
-}.
-
-Fixpoint eq_ctx {T} eqb (C1 : @dy_ctx T) (C2 : @dy_ctx T) :=
+Fixpoint eq_C {T} eqb (C1 C2 : @dy_ctx T) :=
   match C1, C2 with
   | [||], [||] => true
   | dy_binde x1 t1 C1', dy_binde x2 t2 C2' =>
-    eq_eid x1 x2 && eqb t1 t2 && eq_ctx eqb C1' C2'
+    eqb_ID x1 x2 && eqb t1 t2 && eq_C eqb C1' C2'
   | dy_bindm M1 C1' C1'', dy_bindm M2 C2' C2'' =>
-    eq_mid M1 M2 && eq_ctx eqb C1' C2' && eq_ctx eqb C1'' C2''
+    eqb_ID M1 M2 && eq_C eqb C1' C2' && eq_C eqb C1'' C2''
   | _, _ => false
   end.
 
-Lemma eid_refl : forall x, eq_eid x x = true.
-Proof. intros; apply eq_eid_eq; eauto. Qed.
-
-Lemma mid_refl : forall M, eq_mid M M = true.
-Proof. intros; apply eq_mid_eq; eauto. Qed.
-
-Lemma t_refl {T} `{Eq T} : forall t, eqb t t = true.
-Proof. intros; apply eqb_eq; eauto. Qed.
-
 Lemma ctx_refl {T} eqb (t_refl : forall t, eqb t t = true) : 
-  forall (C : @dy_ctx T),
-    eq_ctx eqb C C = true.
+  forall (C : @dy_ctx T), eq_C eqb C C = true.
 Proof.
-  induction C; simpl; try rewrite eid_refl; try rewrite mid_refl;
-  try rewrite t_refl; try rewrite IHC; try rewrite IHC1; try rewrite IHC2; eauto.
+  induction C; simpl; try rewrite ID_refl; try rewrite t_refl;
+  try rewrite IHC; try rewrite IHC1; try rewrite IHC2; eauto.
+Qed.
+
+Lemma eq_C_st_eq {T} eqb (C1 C2 : @dy_ctx T) :
+  eq_C eqb C1 C2 = true -> dy_to_st C1 = dy_to_st C2.
+Proof.
+  intros EQ. revert C2 EQ.
+  induction C1; induction C2; intros; simpl; eauto; try (inversion EQ; fail);
+  simpl in EQ.
+  destruct (eqb_ID x x0) eqn:EQID; try (inversion EQ; fail);
+  destruct (eqb tx tx0) eqn:EQt; try (inversion EQ; fail);
+  destruct (eq_C eqb C1 C2) eqn:EQC; try (inversion EQ; fail).
+  rewrite IHC1 with (C2 := C2); eauto.
+  replace x0 with x; eauto. rewrite <- eqb_ID_eq; eauto.
+  destruct (eqb_ID M M0) eqn:EQID; try (inversion EQ; fail);
+  destruct (eq_C eqb C1_1 C2_1) eqn:EQC1; try (inversion EQ; fail);
+  destruct (eq_C eqb C1_2 C2_2) eqn:EQC2; try (inversion EQ; fail).
+  erewrite IHC1_1; eauto. erewrite IHC1_2; eauto.
+  replace M0 with M. eauto. rewrite <- eqb_ID_eq; eauto.
+Qed.
+
+Lemma eq_C_level_eq {T} eqb (C1 C2 : @dy_ctx T) :
+  eq_C eqb C1 C2 = true -> dy_level C1 = dy_level C2.
+Proof.
+  intros EQ.
+  repeat rewrite st_dy_level_eq.
+  erewrite eq_C_st_eq; eauto.
 Qed.
 
 (* injection, deletion *)
 
-Fixpoint map_inject {T} (Cout : @dy_ctx T) (Cin : @dy_ctx T) :=
+Fixpoint inject {T} (Cout Cin : @dy_ctx T) :=
   match Cin with
-  | [||] => [||]
+  | [||] => Cout
   | dy_binde x t C' =>
-    dy_binde x t (map_inject Cout C')
+    dy_binde x t (inject Cout C')
   | dy_bindm M C' C'' =>
-    dy_bindm M (Cout[|map_inject Cout C'|]) (map_inject Cout C'')
+    dy_bindm M (inject Cout C') (inject Cout C'')
   end.
 
-Definition inject_ctx {T} (Cout : @dy_ctx T) (Cin : @dy_ctx T) :=
-  Cout[|map_inject Cout Cin|].
-
-Fixpoint delete_prefix {T} eqb 
-  (Cout : @dy_ctx T) (Cin : @dy_ctx T) :=
-  match Cout, Cin with
-  | [||], Cin => Cin
-  | dy_binde x t Cout', dy_binde x' t' Cin' =>
-    if eq_eid x x' && eqb t t' then
-      delete_prefix eqb Cout' Cin'
-    else Cin
-  | dy_bindm M Cout' Cout'', dy_bindm M' Cin' Cin'' =>
-    if eq_mid M M' && eq_ctx eqb Cout' Cin' then
-      delete_prefix eqb Cout'' Cin''
-    else Cin
-  | _, _ => Cin
-  end.
-
-Lemma delete_prefix_eq {T} eqb (t_refl : forall t, eqb t t = true) :
-  forall (Cout Cin : @dy_ctx T),
-    delete_prefix eqb Cout (Cout[|Cin|]) = Cin.
-Proof.
-  intros. revert Cin.
-  induction Cout; simpl; eauto;    
-    try rewrite eid_refl; try rewrite mid_refl; try rewrite t_refl; try rewrite ctx_refl;
-    simpl; eauto.
-Qed.
-
-Lemma delete_prefix_dec {T} eqb :
-  forall (Cout Cin : @dy_ctx T),
-    dy_level (delete_prefix eqb Cout Cin) <= dy_level Cin.
-Proof.
-  intros. revert Cout. 
-  induction Cin; intros; destruct Cout; simpl; eauto;
-  try destruct (eq_eid x0 x); try destruct (eqb tx0 tx);
-  try destruct (eq_mid M0 M); try destruct (eq_ctx eqb Cout1 Cin1);
-  simpl; try nia.
-  etransitivity; try apply IHCin; eauto.
-  etransitivity; try apply IHCin; eauto.
-  nia.
-Qed.
-
-Require Import Program.
-
-Program Fixpoint delete_map {T} eqb
-  (Cout Cin : @dy_ctx T) {measure (dy_level Cin)} :=
-  match Cin with
+Fixpoint delete {T} eqb (Cout Cin : @dy_ctx T) :=
+  if eq_C eqb Cout Cin then [||]
+  else match Cin with
   | [||] => [||]
-  | dy_binde x t C' =>
-    dy_binde x t (delete_map eqb Cout C')
-  | dy_bindm M C' C'' =>
-    dy_bindm M (delete_map eqb Cout (delete_prefix eqb Cout C'))
-               (delete_map eqb Cout C'')
+  | dy_binde x t Cin' =>
+    dy_binde x t (delete eqb Cout Cin')
+  | dy_bindm M Cin' Cin'' =>
+    dy_bindm M (delete eqb Cout Cin') (delete eqb Cout Cin'')
   end.
 
-Next Obligation.
-  simpl.
-  pose proof (delete_prefix_dec eqb0 Cout C').
-  nia.
-Defined.
-Next Obligation.
-  simpl.
-  pose proof (delete_prefix_dec eqb0 Cout C'').
-  nia.
-Defined.
-
-(* reduction lemmas *)
-Lemma delete_map_red_binde {T} (eqb : T -> T -> bool) :
-  forall Cout x t C',
-    delete_map eqb Cout (dy_binde x t C') =
-      dy_binde x t (delete_map eqb Cout C').
+Lemma inject_level_inc {T} (Cout Cin : @dy_ctx T) :
+  dy_level Cout <= dy_level (inject Cout Cin).
 Proof.
-  intros. unfold delete_map. unfold delete_map_func.
-  rewrite fix_sub_eq; simpl; try reflexivity.
-  intros x' f g Heq.
-  specialize (functional_extensionality_dep f g Heq).
-  intros RR. rewrite RR. reflexivity.
+  induction Cin; intros; simpl; nia.
 Qed.
-
-Lemma delete_map_red_bindm {T} (eqb : T -> T -> bool) :
-  forall Cout M C' C'',
-    delete_map eqb Cout (dy_bindm M C' C'') =
-      dy_bindm M (delete_map eqb Cout (delete_prefix eqb Cout C'))
-                 (delete_map eqb Cout C'').
-Proof.
-  intros. unfold delete_map. unfold delete_map_func.
-  rewrite fix_sub_eq; simpl; try reflexivity.
-  intros x' f g Heq.
-  specialize (functional_extensionality_dep f g Heq).
-  intros RR. rewrite RR. reflexivity.
-Qed.
-
-Ltac simpl_delete :=
-  simpl;
-  try rewrite delete_map_red_binde;
-  try rewrite delete_map_red_bindm.
-
-Lemma delete_map_eq {T} eqb (t_refl : forall t, eqb t t = true) :
-  forall (Cout Cin : @dy_ctx T),
-    delete_map eqb Cout (map_inject Cout Cin) = Cin.
-Proof.
-  intros. revert Cout.
-  induction Cin; intros; simpl_delete; 
-  try rewrite IHCin; eauto.
-  rewrite delete_prefix_eq. 
-  rewrite IHCin1. rewrite IHCin2. eauto. eauto.
-Qed.
-
-Definition delete_ctx {T} eqb (Cout Cin : @dy_ctx T) :=
-  delete_map eqb Cout (delete_prefix eqb Cout Cin).
 
 Lemma delete_inject_eq {T} eqb (t_refl : forall t, eqb t t = true) :
   forall (Cout Cin : @dy_ctx T),
-    delete_ctx eqb Cout (inject_ctx Cout Cin) = Cin.
+    delete eqb Cout (inject Cout Cin) = Cin.
 Proof.
-  intros. unfold delete_ctx. unfold inject_ctx.
-  rewrite delete_prefix_eq; eauto.
-  rewrite delete_map_eq; eauto.
+  intros. revert Cout. induction Cin; simpl.
+  - induction Cout; eauto;
+    simpl; rewrite ID_refl; try rewrite t_refl; repeat rewrite ctx_refl; eauto.
+  - intros. rewrite IHCin.
+    destruct (eq_C eqb Cout (dy_binde x tx (inject Cout Cin))) eqn:F; eauto.
+    assert (dy_level Cout = dy_level (dy_binde x tx (inject Cout Cin))) as RR.
+    { eapply eq_C_level_eq; eauto. }
+    simpl in RR.
+    pose proof (inject_level_inc Cout Cin) as contra. nia.
+  - intros. rewrite IHCin1. rewrite IHCin2.
+    destruct (eq_C eqb Cout (dy_bindm M (inject Cout Cin1) (inject Cout Cin2))) eqn:F; eauto.
+    assert (dy_level Cout = dy_level (dy_bindm M (inject Cout Cin1) (inject Cout Cin2))) as RR.
+    { eapply eq_C_level_eq; eauto. }
+    simpl in RR.
+    pose proof (inject_level_inc Cout Cin1) as contra1.
+    pose proof (inject_level_inc Cout Cin2) as contra2. nia.
 Qed.
   
-Notation "Cout '<|' Cin '|>'" := (inject_ctx Cout Cin)
-                              (at level 100, Cin at next level, right associativity).
+Notation "Cin '[|' Cout '|]'" := (inject Cout Cin)
+                              (at level 99, Cout at next level, right associativity).
 
-Definition inject_ctx_v {T} `{Eq T} (Cout : @dy_ctx T) (v : @expr_value T) :=
+Definition inject_v {T} `{Eq T} (Cout : @dy_ctx T) (v : @expr_value T) :=
   match v with
-  | Closure x t C => Closure x t (Cout <|C|>)
+  | Closure x t C => Closure x t (Cout [|C|])
   end.
 
-Definition delete_ctx_v {T} eqb (Cout : @dy_ctx T) (v : @expr_value T) :=
+Definition delete_v {T} eqb (Cout : @dy_ctx T) (v : @expr_value T) :=
   match v with
-  | Closure x t C => Closure x t (delete_ctx eqb Cout C)
+  | Closure x t C => Closure x t (delete eqb Cout C)
   end.
 
-Lemma plugin_map_assoc :
-  forall {T} `{Eq T} (Cout C C' : @dy_ctx T),
-    (map_inject Cout C) [|map_inject Cout C'|] = (map_inject Cout (C [|C'|])).
-Proof.
-  intros. revert Cout C'. induction C; intros; simpl; eauto; try rewrite IHC; try rewrite IHC2; eauto.
-Qed.
-
-Lemma plugin_inject_assoc :
-  forall {T} `{Eq T} (Cout C C' : @dy_ctx T),
-    (Cout <| C |>)[| map_inject Cout C' |] = (Cout <|C[|C'|]|>).
-Proof.
-  intros. unfold inject_ctx. rewrite <- c_plugin_assoc.
-  rewrite plugin_map_assoc. eauto.
-Qed.
-
-Lemma map_inject_addr_x :
-  forall {T} `{Eq T} x (Cout : @dy_ctx T) (Cin : @dy_ctx T),
-    addr_x (map_inject Cout Cin) x = addr_x Cin x.
-Proof.
-  intros. revert Cout. 
-  induction Cin; intros; simpl; eauto;
-  destruct (addr_x Cin x) eqn:ADDR;
-  rewrite IHCin; eauto.
-Qed.
-
-Lemma map_inject_ctx_M :
-  forall {T} `{Eq T} M (Cout : @dy_ctx T) (Cin : @dy_ctx T),
-    ctx_M (map_inject Cout Cin) M =
+Lemma inject_ctx_M :
+  forall {T} `{Eq T} M (Cout Cin : @dy_ctx T),
+    ctx_M (Cin [| Cout |]) M =
     match ctx_M Cin M with
-    | Some CM => Some (Cout <| CM |>)
-    | None => None
+    | Some CM => Some (CM [| Cout |])
+    | None => ctx_M Cout M
     end.
 Proof.
   intros. revert Cout.
   induction Cin; intros; simpl; eauto.
-  rewrite IHCin2. destruct (ctx_M Cin2 M); eauto.
-  destruct (eq_mid M M0); eauto.
+  rewrite IHCin2.
+  destruct (eqb_ID M M0); eauto.
 Qed.
 
-Lemma plugin_ctx_addr_x :
-  forall {T} `{Eq T} x (Cout : @dy_ctx T) (Cin : @dy_ctx T),
+Lemma inject_addr_x :
+  forall {T} `{Eq T} x (Cout Cin : @dy_ctx T),
+    addr_x (Cin [| Cout |]) x =
     match addr_x Cin x with
-    | Some t => addr_x (Cout[|Cin|]) x = Some t
-    | None => True
+    | Some t => Some t
+    | None => addr_x Cout x
     end.
 Proof.
-  intros. revert Cin.
-  induction Cout; intros; 
-  destruct (addr_x Cin x) eqn:ADDR; simpl; eauto;
-  try (specialize (IHCout Cin); rewrite ADDR in IHCout;
-      rewrite IHCout; eauto).
-  specialize (IHCout2 Cin); rewrite ADDR in IHCout2; rewrite IHCout2; eauto.
+  intros. revert Cout.
+  induction Cin; intros; simpl; eauto.
+  rewrite IHCin.
+  destruct (eqb_ID x x0); eauto.
 Qed.
 
-Lemma plugin_ctx_ctx_M :
-  forall {T} `{Eq T} M (Cout : @dy_ctx T) (Cin : @dy_ctx T),
-    match ctx_M Cin M with
-    | Some CM => ctx_M (Cout[|Cin|]) M = Some CM
-    | None => True
-    end.
-Proof.
-  intros. revert Cin.
-  induction Cout; intros;
-  destruct (ctx_M Cin M) eqn:CTX; simpl; eauto;
-  try (specialize (IHCout Cin); rewrite CTX in IHCout;
-      rewrite IHCout; eauto).
-  specialize (IHCout2 Cin); rewrite CTX in IHCout2; rewrite IHCout2; eauto.
-Qed.
-
-Lemma inject_ctx_addr_x :
-  forall {T} `{Eq T} x (Cout : @dy_ctx T) (Cin : @dy_ctx T),
-    match addr_x Cin x with
-    | Some t => addr_x (Cout<|Cin|>) x = Some t
-    | None => True
-    end.
-Proof.
-  intros. destruct (addr_x Cin x) eqn:ADDR; eauto.
-  rewrite <- map_inject_addr_x with (Cout := Cout) in ADDR.
-  rewrite <- ADDR. 
-  pose proof plugin_ctx_addr_x.
-  specialize (H0 x Cout (map_inject Cout Cin)).
-  rewrite ADDR in H0. rewrite <- H0 in ADDR.
-  eauto.
-Qed.
-
-Lemma inject_ctx_ctx_M :
-  forall {T} `{Eq T} M (Cout : @dy_ctx T) (Cin : @dy_ctx T),
-    match ctx_M Cin M with
-    | Some CM => ctx_M (Cout<|Cin|>) M = Some (Cout <|CM|>)
-    | None => True
-    end.
-Proof.
-  intros. destruct (ctx_M Cin M) eqn:CTX; eauto.
-  pose proof (map_inject_ctx_M M Cout Cin).
-  rewrite CTX in H0.
-  pose proof (plugin_ctx_ctx_M M Cout (map_inject Cout Cin)).
-  rewrite H0 in H1. eauto.
-Qed.
-
-(* lemmas for trans_ctx *)
-Lemma trans_ctx_id_eq {T} :
-  forall (C : @dy_ctx T), trans_ctx id C = C.
+(* lemmas for trans_C *)
+Lemma trans_C_id_eq {T} :
+  forall (C : @dy_ctx T), trans_C id C = C.
 Proof.
   induction C; simpl; try rewrite IHC; eauto.
   rewrite IHC1. rewrite IHC2. reflexivity.
 Qed.
 
-Lemma eq_ctx_eq {T} `{Eq T} :
+Lemma eq_C_eq {T} `{Eq T} :
   forall (C C' : @dy_ctx T),
-  eq_ctx eqb C C' = true <-> C = C'.
+  eq_C eqb C C' = true <-> C = C'.
 Proof.
   induction C; destruct C'; simpl;
   try (split; intros contra; inversion contra; eauto; fail).
   - split; intros EQ.
-    + destruct (eq_eid x x0) eqn:EQid; try (inversion EQ; fail);
+    + destruct (eqb_ID x x0) eqn:EQid; try (inversion EQ; fail);
       destruct (eqb tx tx0) eqn:EQt; try (inversion EQ; fail).
       simpl in EQ.
-      rewrite IHC in EQ. rewrite eq_eid_eq in EQid. rewrite eqb_eq in EQt.
+      rewrite IHC in EQ. rewrite eqb_ID_eq in EQid. rewrite eqb_eq in EQt.
       subst; eauto.
-    + inversion EQ. subst. rewrite eid_refl. rewrite t_refl. simpl.
+    + inversion EQ. subst. rewrite ID_refl. rewrite t_refl. simpl.
       apply IHC. eauto.
   - split; intros EQ.
-    + destruct (eq_mid M M0) eqn:EQid; try (inversion EQ; fail);
-      destruct (eq_ctx eqb C1 C'1) eqn:EQC1; try (inversion EQ; fail).
+    + destruct (eqb_ID M M0) eqn:EQid; try (inversion EQ; fail);
+      destruct (eq_C eqb C1 C'1) eqn:EQC1; try (inversion EQ; fail).
       simpl in EQ.
-      rewrite IHC2 in EQ. rewrite eq_mid_eq in EQid. rewrite IHC1 in EQC1.
+      rewrite IHC2 in EQ. rewrite eqb_ID_eq in EQid. rewrite IHC1 in EQC1.
       subst; eauto.
-    + inversion EQ. subst. rewrite mid_refl. simpl.
-      replace (eq_ctx eqb C'1 C'1) with true. simpl.
+    + inversion EQ. subst. rewrite ID_refl. simpl.
+      replace (eq_C eqb C'1 C'1) with true. simpl.
       apply IHC2. eauto. symmetry. apply IHC1. eauto.
 Qed.
 
-Lemma trans_ctx_eq_ctx {CT AT} `{ECT : Eq CT} `{EAT : Eq AT} (α : CT -> AT) :
+Lemma trans_C_eq_C {CT AT} `{ECT : Eq CT} `{EAT : Eq AT} (α : CT -> AT) :
   forall C C',
     let eqb' t t' := eqb (α t) (α t') in
-    eq_ctx eqb' C C' = true <->
-    trans_ctx α C = trans_ctx α C'.
+    eq_C eqb' C C' = true <->
+    trans_C α C = trans_C α C'.
 Proof.
-  induction C; induction C'; simpl; try (split; intros contra; inversion contra; eauto; fail).
+  induction C; induction C'; simpl;
+  try (split; intros contra; inversion contra; eauto; fail).
   - split; intros EQ.
-    + destruct (eq_eid x x0) eqn:EQid;
+    + destruct (eqb_ID x x0) eqn:EQid;
       try (inversion EQ; fail).
       destruct (eqb (α tx) (α tx0)) eqn:EQt;
       try (inversion EQ; fail).
-      destruct (eq_ctx (fun t t' : CT => eqb (α t) (α t')) C C') eqn:EQC;
+      destruct (eq_C (fun t t' : CT => eqb (α t) (α t')) C C') eqn:EQC;
       try (inversion EQ; fail).
-      rewrite eq_eid_eq in EQid. rewrite eqb_eq in EQt.
+      rewrite eqb_ID_eq in EQid. rewrite eqb_eq in EQt.
       specialize (IHC C').
       rewrite EQid. rewrite EQt. 
-      replace (trans_ctx α C') with (trans_ctx α C). reflexivity. 
+      replace (trans_C α C') with (trans_C α C). reflexivity. 
       apply IHC. eauto.
-    + inversion EQ; subst. rewrite eid_refl. simpl.
+    + inversion EQ; subst. rewrite ID_refl. simpl.
       rewrite t_refl. simpl.
       rewrite IHC. eauto.
   - split; intros EQ.
-    + destruct (eq_mid M M0) eqn:EQid;
+    + destruct (eqb_ID M M0) eqn:EQid;
       try (inversion EQ; fail).
-      destruct (eq_ctx (fun t t' : CT => eqb (α t) (α t')) C1 C'1) eqn:EQC1;
+      destruct (eq_C (fun t t' : CT => eqb (α t) (α t')) C1 C'1) eqn:EQC1;
       try (inversion EQ; fail).
-      destruct (eq_ctx (fun t t' : CT => eqb (α t) (α t')) C2 C'2) eqn:EQC2;
+      destruct (eq_C (fun t t' : CT => eqb (α t) (α t')) C2 C'2) eqn:EQC2;
       try (inversion EQ; fail).
-      rewrite eq_mid_eq in EQid.
+      rewrite eqb_ID_eq in EQid.
       specialize (IHC1 C'1). specialize (IHC2 C'2).
       rewrite EQid.
-      replace (trans_ctx α C'1) with (trans_ctx α C1).
-      replace (trans_ctx α C'2) with (trans_ctx α C2). reflexivity.
+      replace (trans_C α C'1) with (trans_C α C1).
+      replace (trans_C α C'2) with (trans_C α C2). reflexivity.
       rewrite <- IHC2. eauto. rewrite <- IHC1. eauto.
-    + inversion EQ; subst. rewrite mid_refl. simpl.
-      replace (eq_ctx (fun t t' : CT => eqb (α t) (α t')) C1 C'1) with true. simpl.
+    + inversion EQ; subst. rewrite ID_refl. simpl.
+      replace (eq_C (fun t t' : CT => eqb (α t) (α t')) C1 C'1) with true. simpl.
       rewrite IHC2. eauto. symmetry. rewrite IHC1. eauto.
 Qed.
 
-Lemma trans_ctx_prefix {CT AT} `{ECT : Eq CT} `{EAT : Eq AT} (α : CT -> AT) :
+Lemma trans_C_delete {CT AT} `{ECT : Eq CT} `{EAT : Eq AT} (α : CT -> AT) :
   forall Cout C,
     let eqb' t t' := eqb (α t) (α t') in
-    trans_ctx α (delete_prefix eqb' Cout C) = 
-    delete_prefix eqb (trans_ctx α Cout) (trans_ctx α C).
-Proof.
-  induction Cout; intros; eauto.
-  - simpl. destruct C; eauto.
-    simpl in IHCout. subst eqb'. simpl.
-    destruct (eq_eid x x0) eqn:EQid; destruct (eqb (α tx) (α tx0)) eqn:EQt;
-    simpl; eauto.
-  - simpl. destruct C; eauto.
-    destruct (eq_mid M M0) eqn:EQid; destruct (eq_ctx eqb' Cout1 C1) eqn:EQC;
-    simpl; rewrite EQid; simpl; eauto.
-    apply trans_ctx_eq_ctx in EQC. rewrite EQC.
-    rewrite ctx_refl. eauto. intros. rewrite eqb_eq. eauto.
-    replace (eq_ctx eqb (trans_ctx α Cout1) (trans_ctx α C1)) with false.
-    reflexivity.
-    symmetry. subst eqb'.
-    destruct (eq_ctx eqb (trans_ctx α Cout1) (trans_ctx α C1)) eqn:EQctx; try reflexivity.
-    rewrite trans_ctx_eq_ctx in EQctx. repeat rewrite trans_ctx_id_eq in EQctx.
-    rewrite <- trans_ctx_eq_ctx in EQctx. rewrite EQctx in EQC. inversion EQC.
-Qed.
-
-Lemma trans_ctx_map_aux {CT AT} `{ECT : Eq CT} `{EAT : Eq AT} (α : CT -> AT) :
-  forall n C Cout (LE : dy_level C <= n),
-    let eqb' t t' := eqb (α t) (α t') in
-    trans_ctx α (delete_map eqb' Cout C) = delete_map eqb (trans_ctx α Cout) (trans_ctx α C).
-Proof.
-  induction n; intros; induction C; try reflexivity; try (inversion LE; fail).
-  - rewrite delete_map_red_binde. simpl. rewrite IHn.
-    rewrite delete_map_red_binde. reflexivity. simpl in LE. nia.
-  - rewrite delete_map_red_bindm. simpl. rewrite IHn.
-    rewrite delete_map_red_bindm. rewrite IHC2. 
-    subst eqb'. rewrite trans_ctx_prefix. reflexivity.
-    simpl in LE. nia.
-    etransitivity. apply delete_prefix_dec.
-    simpl in LE. nia.
-Qed.
-
-Lemma trans_ctx_map {CT AT} `{ECT : Eq CT} `{EAT : Eq AT} (α : CT -> AT) :
-  forall Cout C,
-    let eqb' t t' := eqb (α t) (α t') in
-    trans_ctx α (delete_map eqb' Cout C) = delete_map eqb (trans_ctx α Cout) (trans_ctx α C).
+    trans_C α (delete eqb' Cout C) = delete eqb (trans_C α Cout) (trans_C α C).
 Proof.
   intros.
-  apply trans_ctx_map_aux with (n := dy_level C).
-  eauto.
+  assert (forall C', eq_C eqb' Cout C' = eq_C eqb (trans_C α Cout) (trans_C α C')) as RR.
+  { induction Cout; induction C'; eauto.
+    simpl. rewrite IHCout. eauto.
+    simpl. rewrite IHCout1. rewrite IHCout2. eauto. }
+  induction C; intros; simpl; rewrite RR; simpl.
+  - destruct (eq_C eqb (trans_C α Cout) ([||])); eauto.
+  - destruct (eq_C eqb (trans_C α Cout) (dy_binde x (α tx) (trans_C α C))); eauto.
+    simpl. rewrite IHC. eauto.
+  - destruct (eq_C eqb (trans_C α Cout)
+      (dy_bindm M (trans_C α C1) (trans_C α C2))); eauto.
+    simpl. rewrite IHC1. rewrite IHC2. eauto.
 Qed.
-
-Lemma trans_ctx_delete {CT AT} `{ECT : Eq CT} `{EAT : Eq AT} (α : CT -> AT) :
-  forall Cout C,
-    let eqb' t t' := eqb (α t) (α t') in
-    trans_ctx α (delete_ctx eqb' Cout C) = delete_ctx eqb (trans_ctx α Cout) (trans_ctx α C).
-Proof.
-  intros.
-  unfold delete_ctx. subst eqb'.
-  rewrite trans_ctx_map. rewrite trans_ctx_prefix.
-  reflexivity.
-Qed.
-
-(* Typeclass for concrete times *)
-Class OrderT (T : Type) `{Eq T} : Type :=
-{
-  leb : T -> T -> bool;
-  leb_refl : forall t, leb t t = true;
-  leb_trans : forall t t' t'' (LE : leb t t' = true) (LE' : leb t' t'' = true), leb t t'' = true;
-  leb_sym : forall t t' (LE : leb t t' = true) (LE' : leb t' t = true), t = t';
-  leb_or : forall t t', leb t t' || leb t' t = true
-}.
-
-Definition lt {T} `{OrderT T} (t1 t2 : T) :=
-  leb t1 t2 = true /\ eqb t1 t2 = false.
-
-Notation "t1 '<' t2" := (lt t1 t2).
-
-Ltac contradict :=
-  let contra := fresh "contra" in
-  assert False as contra; eauto 3; inversion contra.
-
-Lemma __R__ : forall b, b = false <-> ~ b = true.
-Proof. 
-  intros; destruct b; unfold "<>"; split; 
-  intros; try inversion H; try inversion H0; try contradict; eauto.
-Qed.
-
-Ltac refl_bool :=
-  match goal with
-  | |- _ = false => rewrite __R__; unfold "<>"
-  | |- _ <> true => rewrite <- __R__
-  | _ => idtac
-  end.
